@prefix : <http://purl.oclc.org/NET/ssnx/qu/qu#> .
@prefix cc: <http://creativecommons.org/ns#> .
@prefix dc: <http://purl.org/dc/elements/1.1/> .
@prefix qu: <http://purl.oclc.org/NET/ssnx/qu/qu#> .
@prefix dct: <http://purl.org/dc/terms/> .
@prefix dim: <http://purl.oclc.org/NET/ssnx/qu/dim#> .
@prefix owl: <http://www.w3.org/2002/07/owl#> .
@prefix rdf: <http://www.w3.org/1999/02/22-rdf-syntax-ns#> .
@prefix xml: <http://www.w3.org/XML/1998/namespace> .
@prefix xsd: <http://www.w3.org/2001/XMLSchema#> .
@prefix rdfs: <http://www.w3.org/2000/01/rdf-schema#> .
@prefix skos: <http://www.w3.org/2004/02/skos/core#> .
@prefix unit: <http://purl.oclc.org/NET/ssnx/qu/unit#> .
@prefix prefix: <http://purl.oclc.org/NET/ssnx/qu/prefix#> .
@prefix quantity: <http://purl.oclc.org/NET/ssnx/qu/quantity#> .
@base <http://purl.oclc.org/NET/ssnx/qu/qu> .

<http://purl.oclc.org/NET/ssnx/qu/qu> rdf:type owl:Ontology ;
                                      
                                      rdfs:comment ""^^xsd:string ;
                                      
                                      dc:creator "Hans Peter de Koning (ESA, Netherlands and QUDV working group of the SysML 1.2 Revision Task Force (RTF))"^^xsd:string ,
                                                 "Huascar Espinoza (CEA, France and QUDV working group of the SysML 1.2 Revision Task Force (RTF))"^^xsd:string ;
                                      
                                      rdfs:comment "In order to generalize its potential usage and alignment with other standardization efforts concerning quantities and units, the QU  ontology has been further developed as a complement to the Agriculture Meteorology example showcasing the ontology developed by the W3C Semantic Sensor Networks incubator group (SSN-XG). The Agriculture Meteorology example also includes an application of the QU schema to the UN/CEFACT Recommendation 20 code list. For more information on the group's activities see: http://www.w3.org/2005/Incubator/ssn/ ."^^xsd:string ;
                                      
                                      dc:creator "Laurent Lefort (CSIRO, Australia and W3C Semantic Sensor Network Incubator Group)"^^xsd:string ,
                                                 "Nicolas Rouquette (NASA-JPL, USA and QUDV working group of the SysML 1.2 Revision Task Force (RTF))"^^xsd:string ;
                                      
                                      rdfs:comment "Please report any errors to the Semantic Sensor Network Incubator Activity via the public W3C list public-xg-ssn@w3.org or alternatively, for enquiries about the QUDV model,  to the QUDV mailing list: http://www.omg.org/publicarchives/qudv/"^^xsd:string ;
                                      
                                      dc:creator "Roger Burkhart (John Deere, USA and QUDV working group of the SysML 1.2 Revision Task Force (RTF))"^^xsd:string ;
                                      
                                      rdfs:comment "The QUDV copyright holders have agreed for the QU ontology to be published by the W3C Semantic Sensor Incubator Group but this does not constitute an endorsement or recommendation by the QUDV working group of the SysML 1.2 Revision Task Force. All other rights reserved."^^xsd:string ,
                                                   "This Model Library for Quantities, Units, Dimensions and Values (QUDV)  (Note: in the ontology, the SYSML-QUDV definitions are flagged with a rdfs:seeAlso annotation equal to http://www.omgsysml.org/qudv)."^^xsd:string ,
                                                   """This ontology is partially based on the SysML QUDV (Quantities, Units, Dimensions and Values) proposed by a working group of the SysML 1.2 Revision Task Force (RTF), working in close coordination with the OMG MARTE specification group. This model library is specified in a UML/SysML class/block diagram in the OMG SysML, Version 1.2 specification (http://www.omg.org/spec/SysML/1.2/). This model is described in OMG  SysML, Version 1.2 Appendix C.4 Model Library for Quantity Kinds and Units (http://ontolog.cim3.net/file/resource/reference/UoM_Ontology_Standard/available-UoM-references/QUDV-Annex-C4-C5--OMG-SysML-v1-2_Oct-2009.pdf).		
	
The QUDV model has also been represented in the form of an ontology using a formal ontology definition language. The resulting OWL ontology, called the QUDV ontology http://www.omgwiki.org/OMGSysML/doku.php?id=sysml-qudv:qudv_owl has been published by members of the QUDV working group of the SysML 1.2 Revision Task Force (RTF). 

		OMG SysML is a trademark of OMG (see http://www.omg.org/spec/SysML/1.2/PDF/ for the conditions of use of the  OMG  SysML, Version 1.2  specification).
		"""^^xsd:string ;
                                      
                                      dc:title "Library for Quantity Kinds and Units: schema, based on QUDV model OMG SysML(TM), Version 1.2" ;
                                      
                                      dc:rights "qu.owl  Copyright 2010 - 2011 CSIRO" ;
                                      
                                      dct:created "2009-08-26" ;
                                      
                                      rdfs:seeAlso "http://www.w3.org/2005/Incubator/ssn/" ;
                                      
                                      dc:rights "sysml-qudv:qudv_owl  Copyright 2009 - 2011 The QUDV authors" ;
                                      
                                      dc:identifier "http://purl.oclc.org/NET/ssnx/qu/qu" ;
                                      
                                      dct:modified "2011-06-20" .


#################################################################
#
#    Annotation properties
#
#################################################################


###  http://creativecommons.org/ns#license

cc:license rdf:type owl:AnnotationProperty .



###  http://purl.org/dc/elements/1.1/author

dc:author rdf:type owl:AnnotationProperty .



###  http://purl.org/dc/elements/1.1/creator

dc:creator rdf:type owl:AnnotationProperty .



###  http://purl.org/dc/elements/1.1/description

dc:description rdf:type owl:AnnotationProperty .



###  http://purl.org/dc/elements/1.1/identifier

dc:identifier rdf:type owl:AnnotationProperty .



###  http://purl.org/dc/elements/1.1/rights

dc:rights rdf:type owl:AnnotationProperty .



###  http://purl.org/dc/elements/1.1/source

dc:source rdf:type owl:AnnotationProperty .



###  http://purl.org/dc/elements/1.1/title

dc:title rdf:type owl:AnnotationProperty .



###  http://purl.org/dc/terms/created

dct:created rdf:type owl:AnnotationProperty .



###  http://purl.org/dc/terms/modified

dct:modified rdf:type owl:AnnotationProperty .



###  http://www.w3.org/2000/01/rdf-schema#comment

rdfs:comment rdf:type owl:AnnotationProperty .



###  http://www.w3.org/2000/01/rdf-schema#isDefinedBy

rdfs:isDefinedBy rdf:type owl:AnnotationProperty .



###  http://www.w3.org/2000/01/rdf-schema#label

rdfs:label rdf:type owl:AnnotationProperty .



###  http://www.w3.org/2000/01/rdf-schema#seeAlso

rdfs:seeAlso rdf:type owl:AnnotationProperty .





#################################################################
#
#    Object Properties
#
#################################################################


###  http://purl.oclc.org/NET/ssnx/qu/qu#baseDimension

:baseDimension rdf:type owl:ObjectProperty ;
               
               rdfs:label "baseDimension" ;
               
               rdfs:seeAlso "http://www.omgsysml.org/qudv#Dimension" ;
               
               rdfs:isDefinedBy "http://purl.oclc.org/NET/ssnx/qu" ;
               
               dc:source "skos:exactMatch 'baseDimension' [SysML 1.2-QUDV] http://www.omgwiki.org/OMGSysML/doku.php?id=sysml-qudv:quantities_units_dimensions_values_qudv" ;
               
               rdfs:comment "A Reference to the QuantityKind that represents the base quantity dimension in the factor." ;
               
               rdfs:range :QuantityKind .



###  http://purl.oclc.org/NET/ssnx/qu/qu#baseQuantityKind

:baseQuantityKind rdf:type owl:AsymmetricProperty ,
                           owl:ObjectProperty ;
                  
                  rdfs:label "baseQuantityKind" ;
                  
                  rdfs:comment "Ordered set of QuantityKind that specifies the base quantities of the system of quantities. This is a subset of the complete quantityKind list. The base quantities define the basis for the quantity dimension of a kind of quantity." ;
                  
                  rdfs:seeAlso "http://www.omgsysml.org/qudv#Dimension" ;
                  
                  dc:source "skos:exactMatch 'baseQuantityKind' [SysML 1.2-QUDV] http://www.omgwiki.org/OMGSysML/doku.php?id=sysml-qudv:quantities_units_dimensions_values_qudv" ;
                  
                  rdfs:isDefinedBy "http://purl.oclc.org/NET/ssnx/qu" ;
                  
                  rdfs:range :QuantityKind ;
                  
                  rdfs:subPropertyOf :quantityKind .



###  http://purl.oclc.org/NET/ssnx/qu/qu#baseUnit

:baseUnit rdf:type owl:AsymmetricProperty ,
                   owl:ObjectProperty ;
          
          rdfs:label "baseUnit" ;
          
          rdfs:comment "Ordered set of Unit that specifies the base units of the system of units. A \"base unit\" is defined in [VIM] as a \"measurement unit that is adopted by convention for a base quantity,\" i.e. it is the (preferred) unit in which base quantities of the associated systemOfQuantities are expressed." ;
          
          rdfs:seeAlso "http://www.omgsysml.org/qudv#Dimension" ;
          
          dc:source "skos:exactMatch 'baseUnit' [SysML 1.2-QUDV] http://www.omgwiki.org/OMGSysML/doku.php?id=sysml-qudv:quantities_units_dimensions_values_qudv" ;
          
          rdfs:isDefinedBy "http://purl.oclc.org/NET/ssnx/qu" ;
          
          rdfs:range :Unit ;
          
          rdfs:subPropertyOf :unit .



###  http://purl.oclc.org/NET/ssnx/qu/qu#dimension

:dimension rdf:type owl:ObjectProperty ;
           
           rdfs:label "dimension" ;
           
           rdfs:seeAlso "http://www.omgsysml.org/qudv#Quantity" ;
           
           rdfs:isDefinedBy "http://purl.oclc.org/NET/ssnx/qu" ;
           
           rdfs:comment "Derived ordered set of Dimension. The actual dimension of a QuantityKind depends on the list of baseQuantityKind that are specified in an actual SystemOfQuantities, see the DerivedDimensions constraint." ;
           
           dc:source "skos:exactMatch 'dimension' [SysML 1.2-QUDV] http://www.omgwiki.org/OMGSysML/doku.php?id=sysml-qudv:quantities_units_dimensions_values_qudv" ;
           
           rdfs:range :Dimension .



###  http://purl.oclc.org/NET/ssnx/qu/qu#dimensionFactor

:dimensionFactor rdf:type owl:AsymmetricProperty ,
                          owl:ObjectProperty ;
                 
                 rdfs:label "dimension factor" ;
                 
                 rdfs:isDefinedBy "http://purl.oclc.org/NET/ssnx/qu" ;
                 
                 rdfs:seeAlso "http://www.omgsysml.org/qudv#Dimension" ;
                 
                 rdfs:comment "Rational number that specifies the factor in the dimension conversion relationship." ;
                 
                 dc:source "skos:exactMatch 'factor' [SysML 1.2-QUDV] http://www.omgwiki.org/OMGSysML/doku.php?id=sysml-qudv:quantities_units_dimensions_values_qudv" ;
                 
                 rdfs:range :DimensionFactor .



###  http://purl.oclc.org/NET/ssnx/qu/qu#factorQuantityKind

:factorQuantityKind rdf:type owl:AsymmetricProperty ,
                             owl:ObjectProperty ;
                    
                    rdfs:label "factorQuantityKind" ;
                    
                    dc:source "skos:exactMatch 'quantityKind' [SysML 1.2-QUDV] http://www.omgwiki.org/OMGSysML/doku.php?id=sysml-qudv:quantities_units_dimensions_values_qudv" ;
                    
                    rdfs:isDefinedBy "http://purl.oclc.org/NET/ssnx/qu" ;
                    
                    rdfs:seeAlso "http://www.omgsysml.org/qudv#Quantity" ;
                    
                    rdfs:comment "Specification of the associated QuantityKind." ;
                    
                    rdfs:range :QuantityKind .



###  http://purl.oclc.org/NET/ssnx/qu/qu#generalQuantityKind

:generalQuantityKind rdf:type owl:IrreflexiveProperty ,
                              owl:ObjectProperty ;
                     
                     rdfs:label "generalQuantityKind" ;
                     
                     rdfs:seeAlso "http://www.omgsysml.org/qudv#Quantity" ;
                     
                     dc:source "skos:exactMatch 'generalization' [QUDT] http:qudt.org" ;
                     
                     rdfs:comment "A generalization relationship between two kinds of quantities." ;
                     
                     rdfs:isDefinedBy "http://purl.oclc.org/NET/ssnx/qu" ;
                     
                     dc:source "skos:exactMatch 'general' [SysML 1.2-QUDV] http://www.omgwiki.org/OMGSysML/doku.php?id=sysml-qudv:quantities_units_dimensions_values_qudv" ;
                     
                     rdfs:range :QuantityKind .



###  http://purl.oclc.org/NET/ssnx/qu/qu#prefix

:prefix rdf:type owl:AsymmetricProperty ,
                 owl:IrreflexiveProperty ,
                 owl:ObjectProperty ;
        
        rdfs:label "prefix" ;
        
        rdfs:comment "Ordered set of Prefix that specifies the prefixes for multiples and submultiples of units in the system" ;
        
        rdfs:isDefinedBy "http://purl.oclc.org/NET/ssnx/qu" ;
        
        dc:source "skos:exactMatch 'prefix' [SysML 1.2-QUDV] http://www.omgwiki.org/OMGSysML/doku.php?id=sysml-qudv:quantities_units_dimensions_values_qudv" ;
        
        rdfs:seeAlso "http://www.omgsysml.org/qudv#Unit" ;
        
        rdfs:range :Prefix .



###  http://purl.oclc.org/NET/ssnx/qu/qu#propertyType

:propertyType rdf:type owl:AsymmetricProperty ,
                       owl:ObjectProperty ;
              
              rdfs:label "propertyType" ;
              
              rdfs:isDefinedBy "http://purl.oclc.org/NET/ssnx/qu" ;
              
              rdfs:comment "Specification of the associated ProeprtyType." ;
              
              rdfs:seeAlso "http://www.omgsysml.org/qudv#Quantity" ;
              
              rdfs:range :PropertyKind .



###  http://purl.oclc.org/NET/ssnx/qu/qu#quantityComponent

:quantityComponent rdf:type owl:AsymmetricProperty ,
                            owl:ObjectProperty ;
                   
                   rdfs:label "quantityComponent" ;
                   
                   rdfs:isDefinedBy "http://purl.oclc.org/NET/ssnx/qu" ;
                   
                   dc:source "skos:exactMatch 'quantityKind' [SysML 1.2-QUDV] http://www.omgwiki.org/OMGSysML/doku.php?id=sysml-qudv:quantities_units_dimensions_values_qudv" ;
                   
                   rdfs:comment "Quantities attached to a system." ;
                   
                   rdfs:seeAlso "http://www.omgsysml.org/qudv#Dimension" ;
                   
                   rdfs:range :QuantityKind .



###  http://purl.oclc.org/NET/ssnx/qu/qu#quantityKind

:quantityKind rdf:type owl:AsymmetricProperty ,
                       owl:ObjectProperty ;
              
              rdfs:label "quantityKind" ;
              
              rdfs:comment "Specification of the associated QuantityKind." ;
              
              rdfs:seeAlso "http://www.omgsysml.org/qudv#Quantity" ;
              
              dc:source "skos:exactMatch 'quantityKind' [SysML 1.2-QUDV] http://www.omgwiki.org/OMGSysML/doku.php?id=sysml-qudv:quantities_units_dimensions_values_qudv" ;
              
              rdfs:isDefinedBy "http://purl.oclc.org/NET/ssnx/qu" ;
              
              rdfs:range :QuantityKind .



###  http://purl.oclc.org/NET/ssnx/qu/qu#quantityKindFactor

:quantityKindFactor rdf:type owl:AsymmetricProperty ,
                             owl:ObjectProperty ;
                    
                    rdfs:label "quantity kind factor" ;
                    
                    rdfs:comment "Rational number that specifies the factor in the quantity conversion relationship." ;
                    
                    rdfs:seeAlso "http://www.omgsysml.org/qudv#Quantity" ;
                    
                    rdfs:isDefinedBy "http://purl.oclc.org/NET/ssnx/qu" ;
                    
                    dc:source "skos:exactMatch 'factor' [SysML 1.2-QUDV] http://www.omgwiki.org/OMGSysML/doku.php?id=sysml-qudv:quantities_units_dimensions_values_qudv" ;
                    
                    rdfs:range :QuantityKindFactor .



###  http://purl.oclc.org/NET/ssnx/qu/qu#referenceUnit

:referenceUnit rdf:type owl:AsymmetricProperty ,
                        owl:ObjectProperty ;
               
               rdfs:label "referenceUnit" ;
               
               dc:source "skos:exactMatch 'referenceUnit' [SysML 1.2-QUDV] http://www.omgwiki.org/OMGSysML/doku.php?id=sysml-qudv:quantities_units_dimensions_values_qudv" ;
               
               rdfs:comment "Specifies the unit with respect to which the ConversionBasedUnit is defined." ;
               
               rdfs:seeAlso "http://www.omgsysml.org/qudv#Unit" ;
               
               rdfs:isDefinedBy "http://purl.oclc.org/NET/ssnx/qu" ;
               
               rdfs:range :Unit .



###  http://purl.oclc.org/NET/ssnx/qu/qu#scale

:scale rdf:type owl:AsymmetricProperty ,
                owl:IrreflexiveProperty ,
                owl:ObjectProperty ;
       
       rdfs:label "scale" ;
       
       dc:source "skos:exactMatch 'scale' [SysML 1.2-QUDV] http://www.omgwiki.org/OMGSysML/doku.php?id=sysml-qudv:quantities_units_dimensions_values_qudv" ;
       
       rdfs:comment "Specification of a Scale that is associated to the QuantityKind." ;
       
       rdfs:seeAlso "http://www.omgsysml.org/qudv#Scale" ;
       
       rdfs:isDefinedBy "http://purl.oclc.org/NET/ssnx/qu" ;
       
       rdfs:range :Scale .



###  http://purl.oclc.org/NET/ssnx/qu/qu#scaleValueDefinition

:scaleValueDefinition rdf:type owl:AsymmetricProperty ,
                               owl:IrreflexiveProperty ,
                               owl:ObjectProperty ;
                      
                      rdfs:label "scaleValueDefinition" ;
                      
                      rdfs:comment "Ordered set of ScaleValueDefinition that specifies the defined numerical value(s) and textual definition(s) for the measurement scale." ;
                      
                      dc:source "skos:exactMatch 'valueDefinition' [SysML 1.2-QUDV] http://www.omgwiki.org/OMGSysML/doku.php?id=sysml-qudv:quantities_units_dimensions_values_qudv" ;
                      
                      rdfs:seeAlso "http://www.omgsysml.org/qudv#Scale" ;
                      
                      rdfs:isDefinedBy "http://purl.oclc.org/NET/ssnx/qu" ;
                      
                      rdfs:range :ScaleValueDefinition .



###  http://purl.oclc.org/NET/ssnx/qu/qu#specificQuantityKind

:specificQuantityKind rdf:type owl:IrreflexiveProperty ,
                               owl:ObjectProperty ;
                      
                      rdfs:label "specificQuantityKind" ;
                      
                      dc:source "skos:exactMatch 'specific' [SysML 1.2-QUDV] http://www.omgwiki.org/OMGSysML/doku.php?id=sysml-qudv:quantities_units_dimensions_values_qudv" ;
                      
                      rdfs:isDefinedBy "http://purl.oclc.org/NET/ssnx/qu" ;
                      
                      rdfs:seeAlso "http://www.omgsysml.org/qudv#Quantity" ;
                      
                      rdfs:comment "A specialization relationship between two kinds of quantities." ;
                      
                      rdfs:range :QuantityKind ,
                                 :SpecializedQuantityKind ;
                      
                      owl:inverseOf :generalQuantityKind .



###  http://purl.oclc.org/NET/ssnx/qu/qu#systemOfQuantities

:systemOfQuantities rdf:type owl:ObjectProperty ;
                    
                    rdfs:label "systemOfQuantities" ;
                    
                    rdfs:seeAlso "http://www.omgsysml.org/qudv#Dimension" ;
                    
                    rdfs:isDefinedBy "http://purl.oclc.org/NET/ssnx/qu" ;
                    
                    rdfs:comment "Reference to the SystemOfQuantities for which the units are specified." ;
                    
                    dc:source "skos:exactMatch 'systemOfQuantities' [SysML 1.2-QUDV] http://www.omgwiki.org/OMGSysML/doku.php?id=sysml-qudv:quantities_units_dimensions_values_qudv" ;
                    
                    rdfs:range :SystemOfQuantities .



###  http://purl.oclc.org/NET/ssnx/qu/qu#unit

:unit rdf:type owl:AsymmetricProperty ,
               owl:ObjectProperty ;
      
      rdfs:label "unit" ;
      
      rdfs:isDefinedBy "http://purl.oclc.org/NET/ssnx/qu" ;
      
      dc:source "skos:exactMatch 'quantityKind' [SysML 1.2-QUDV] http://www.omgwiki.org/OMGSysML/doku.php?id=sysml-qudv:quantities_units_dimensions_values_qudv" ;
      
      rdfs:comment "Specification of the associated Unit." ;
      
      rdfs:seeAlso "http://www.omgsysml.org/qudv#Unit" ;
      
      rdfs:range :Unit .



###  http://purl.oclc.org/NET/ssnx/qu/qu#unitComponent

:unitComponent rdf:type owl:AsymmetricProperty ,
                        owl:ObjectProperty ;
               
               rdfs:label "unitComponent" ;
               
               dc:source "skos:exactMatch 'unit' [SysML 1.2-QUDV] http://www.omgwiki.org/OMGSysML/doku.php?id=sysml-qudv:quantities_units_dimensions_values_qudv" ;
               
               rdfs:isDefinedBy "http://purl.oclc.org/NET/ssnx/qu" ;
               
               rdfs:seeAlso "http://www.omgsysml.org/qudv#Dimension" ;
               
               rdfs:comment "Ordered set of Unit that specifies the units that are known in the system." ;
               
               rdfs:range :Unit .



###  http://purl.oclc.org/NET/ssnx/qu/qu#unitFactor

:unitFactor rdf:type owl:AsymmetricProperty ,
                     owl:ObjectProperty ;
            
            rdfs:label "unit factor" ;
            
            rdfs:comment "Rational number that specifies the factor in the unit conversion relationship." ;
            
            rdfs:isDefinedBy "http://purl.oclc.org/NET/ssnx/qu" ;
            
            rdfs:seeAlso "http://www.omgsysml.org/qudv#Unit" ;
            
            dc:source "skos:exactMatch 'factor' [SysML 1.2-QUDV] http://www.omgwiki.org/OMGSysML/doku.php?id=sysml-qudv:quantities_units_dimensions_values_qudv" ;
            
            rdfs:range :UnitFactor .



###  http://purl.oclc.org/NET/ssnx/qu/qu#unitKind

:unitKind rdf:type owl:AsymmetricProperty ,
                   owl:ObjectProperty ;
          
          rdfs:label "unitKind" ;
          
          rdfs:seeAlso "http://www.omgsysml.org/qudv#Unit" ;
          
          rdfs:comment "Specification of the associated Unit \"Kind\"." ;
          
          rdfs:isDefinedBy "http://purl.oclc.org/NET/ssnx/qu" ;
          
          rdfs:range :Unit ;
          
          owl:inverseOf :quantityKind .





#################################################################
#
#    Data properties
#
#################################################################


###  http://purl.oclc.org/NET/ssnx/qu/qu#code

:code rdf:type owl:DatatypeProperty ;
      
      rdfs:label "code" ;
      
      dc:description "short symbolic name"^^xsd:string ;
      
      rdfs:isDefinedBy "http://purl.oclc.org/NET/ssnx/qu" ;
      
      rdfs:seeAlso "http://www.omgsysml.org/qudv#Data" ;
      
      rdfs:comment "A code is a string that uniquely identifies an individual." ;
      
      dc:source "skos:closeMatch 'code' [QUDT] http://qudt.org/" ;
      
      rdfs:range xsd:string .



###  http://purl.oclc.org/NET/ssnx/qu/qu#conversionFactor

:conversionFactor rdf:type owl:DatatypeProperty ;
                  
                  rdfs:label "conversionFactor" ;
                  
                  dc:source "skos:exactMatch 'factor' [SysML 1.2-QUDV] http://www.omgwiki.org/OMGSysML/doku.php?id=sysml-qudv:quantities_units_dimensions_values_qudv" ;
                  
                  rdfs:comment "Rational number that specifies the factor in the unit conversion relationship." ;
                  
                  rdfs:seeAlso "http://www.omgsysml.org/qudv#Data" ;
                  
                  rdfs:isDefinedBy "http://purl.oclc.org/NET/ssnx/qu" ;
                  
                  rdfs:range xsd:double .



###  http://purl.oclc.org/NET/ssnx/qu/qu#conversionOffset

:conversionOffset rdf:type owl:DatatypeProperty ;
                  
                  rdfs:label "conversionOffset" ;
                  
                  rdfs:comment "Rational number that specifies the offset in the unit conversion relationship." ;
                  
                  rdfs:seeAlso "http://www.omgsysml.org/qudv#Data" ;
                  
                  dc:source "skos:exactMatch 'offset' [SysML 1.2-QUDV] http://www.omgwiki.org/OMGSysML/doku.php?id=sysml-qudv:quantities_units_dimensions_values_qudv" ;
                  
                  rdfs:isDefinedBy "http://purl.oclc.org/NET/ssnx/qu" ;
                  
                  rdfs:range xsd:double .



###  http://purl.oclc.org/NET/ssnx/qu/qu#definitionURI

:definitionURI rdf:type owl:DatatypeProperty ,
                        owl:FunctionalProperty ;
               
               rdfs:label "definitionURI" ;
               
               dc:description "URI that contains an authoritative definition of the referent thing"^^xsd:string ;
               
               rdfs:comment "URI that references an external definition." ;
               
               dc:source "skos:exactMatch 'definitionURI' [SysML 1.2-QUDV] http://www.omgwiki.org/OMGSysML/doku.php?id=sysml-qudv:quantities_units_dimensions_values_qudv" ;
               
               rdfs:isDefinedBy "http://purl.oclc.org/NET/ssnx/qu" ;
               
               rdfs:seeAlso "http://www.omgsysml.org/qudv#Data" ;
               
               rdfs:range xsd:string .



###  http://purl.oclc.org/NET/ssnx/qu/qu#description

:description rdf:type owl:DatatypeProperty ;
             
             rdfs:label "description" ;
             
             rdfs:seeAlso "http://www.omgsysml.org/qudv#Data" ;
             
             dc:source "skos:exactMatch 'description' [SysML 1.2-QUDV] http://www.omgwiki.org/OMGSysML/doku.php?id=sysml-qudv:quantities_units_dimensions_values_qudv" ;
             
             rdfs:comment "Textual description" ;
             
             rdfs:isDefinedBy "http://purl.oclc.org/NET/ssnx/qu" ;
             
             rdfs:range xsd:string .



###  http://purl.oclc.org/NET/ssnx/qu/qu#exponent

:exponent rdf:type owl:DatatypeProperty ;
          
          rdfs:label "exponent" ;
          
          rdfs:seeAlso "http://www.omgsysml.org/qudv#Data" ;
          
          rdfs:isDefinedBy "http://purl.oclc.org/NET/ssnx/qu" ;
          
          rdfs:comment "Rational number that specifies the exponent of the power to which the unit is raised." ;
          
          dc:source "skos:exactMatch 'exponent' [SysML 1.2-QUDV] http://www.omgwiki.org/OMGSysML/doku.php?id=sysml-qudv:quantities_units_dimensions_values_qudv" ;
          
          rdfs:range xsd:double .



###  http://purl.oclc.org/NET/ssnx/qu/qu#expression

:expression rdf:type owl:DatatypeProperty ;
            
            rdfs:label "conversionExpression" ;
            
            rdfs:isDefinedBy "http://purl.oclc.org/NET/ssnx/qu" ;
            
            rdfs:comment "Specifies the unit conversion relationship in some expression syntax." ;
            
            dc:source "skos:exactMatch 'expression' [SysML 1.2-QUDV] http://www.omgwiki.org/OMGSysML/doku.php?id=sysml-qudv:quantities_units_dimensions_values_qudv" ;
            
            rdfs:seeAlso "http://www.omgsysml.org/qudv#Data" ;
            
            rdfs:range xsd:string .



###  http://purl.oclc.org/NET/ssnx/qu/qu#name

:name rdf:type owl:DatatypeProperty ,
               owl:FunctionalProperty ;
      
      rdfs:label "name" ;
      
      dc:description "human-readable word or sequence of words by which a thing is known"^^xsd:string ;
      
      dc:source "skos:exactMatch 'name' [SysML 1.2-QUDV] http://www.omgwiki.org/OMGSysML/doku.php?id=sysml-qudv:quantities_units_dimensions_values_qudv" ;
      
      rdfs:isDefinedBy "http://purl.oclc.org/NET/ssnx/qu" ;
      
      rdfs:seeAlso "http://www.omgsysml.org/qudv#Data" ;
      
      rdfs:range xsd:string .



###  http://purl.oclc.org/NET/ssnx/qu/qu#numericalValue

:numericalValue rdf:type owl:DatatypeProperty ;
                
                rdfs:label "numericalValue" ;
                
                dc:source "skos:exactMatch 'value' [SysML 1.2-QUDV] http://www.omgwiki.org/OMGSysML/doku.php?id=sysml-qudv:quantities_units_dimensions_values_qudv" ;
                
                rdfs:comment "Specifies the numerical value." ;
                
                rdfs:seeAlso "http://www.omgsysml.org/qudv#Data" ;
                
                rdfs:isDefinedBy "http://purl.oclc.org/NET/ssnx/qu" ;
                
                rdfs:range xsd:double .



###  http://purl.oclc.org/NET/ssnx/qu/qu#symbol

:symbol rdf:type owl:DatatypeProperty ;
        
        rdfs:label "symbol" ;
        
        dc:description "short symbolic name"^^xsd:string ;
        
        rdfs:comment "Short symbolic name." ;
        
        rdfs:isDefinedBy "http://purl.oclc.org/NET/ssnx/qu" ;
        
        rdfs:seeAlso "http://www.omgsysml.org/qudv#Data" ;
        
        dc:source "skos:exactMatch 'symbol' [SysML 1.2-QUDV] http://www.omgwiki.org/OMGSysML/doku.php?id=sysml-qudv:quantities_units_dimensions_values_qudv" ;
        
        rdfs:range xsd:string .



###  http://purl.oclc.org/NET/ssnx/qu/qu#symbolicExpression

:symbolicExpression rdf:type owl:DatatypeProperty ;
                    
                    rdfs:label "symbolicExpression" ;
                    
                    rdfs:comment "Symbolic expression of the quantity dimension's product of powers, in terms of symbols of the kinds of quantity that represent the base kinds of quantity and their exponents." ;
                    
                    rdfs:isDefinedBy "http://purl.oclc.org/NET/ssnx/qu" ;
                    
                    dc:source "skos:exactMatch 'symbolicExpression' [SysML 1.2-QUDV] http://www.omgwiki.org/OMGSysML/doku.php?id=sysml-qudv:quantities_units_dimensions_values_qudv" ;
                    
                    rdfs:seeAlso "http://www.omgsysml.org/qudv#Data" ;
                    
                    rdfs:range xsd:string .



###  http://purl.oclc.org/NET/ssnx/qu/qu#unitMultipleFactor

:unitMultipleFactor rdf:type owl:DatatypeProperty ,
                             owl:FunctionalProperty ;
                    
                    rdfs:label "unitMultipleFactor" ;
                    
                    rdfs:isDefinedBy "http://purl.oclc.org/NET/ssnx/qu" ;
                    
                    rdfs:seeAlso "http://www.omgsysml.org/qudv#Data" ;
                    
                    rdfs:comment "Specifies the multiple or submultiple multiplication factor." ;
                    
                    dc:source "skos:exactMatch 'factor' [SysML 1.2-QUDV] http://www.omgwiki.org/OMGSysML/doku.php?id=sysml-qudv:quantities_units_dimensions_values_qudv" ;
                    
                    rdfs:range xsd:double .





#################################################################
#
#    Classes
#
#################################################################


###  http://purl.oclc.org/NET/ssnx/qu/qu#ConversionBasedUnit

:ConversionBasedUnit rdf:type owl:Class ;
                     
                     rdfs:label "ConversionBasedUnit" ;
                     
                     rdfs:subClassOf :Unit ,
                                     [ rdf:type owl:Restriction ;
                                       owl:onProperty :referenceUnit ;
                                       owl:onClass :Unit ;
                                       owl:qualifiedCardinality "1"^^xsd:nonNegativeInteger
                                     ] ;
                     
                     dc:source "skos:exactMatch 'ConversionBasedUnit' [SysML 1.2-QUDV] http://www.omgwiki.org/OMGSysML/doku.php?id=sysml-qudv:quantities_units_dimensions_values_qudv" ;
                     
                     rdfs:comment """A ConversionBasedUnit is an abstract classifier that is a Unit that represents a measurement unit that is defined with respect to
another reference unit through an explicit conversion relationship.""" ;
                     
                     rdfs:seeAlso "http://www.omgsysml.org/qudv#Unit" ;
                     
                     rdfs:isDefinedBy "http://purl.oclc.org/NET/ssnx/qu" .



###  http://purl.oclc.org/NET/ssnx/qu/qu#DerivedQuantityKind

:DerivedQuantityKind rdf:type owl:Class ;
                     
                     rdfs:label "DerivedQuantityKind" ;
                     
                     rdfs:subClassOf :QuantityKind ,
                                     [ rdf:type owl:Restriction ;
                                       owl:onProperty :quantityKindFactor ;
                                       owl:someValuesFrom :QuantityKindFactor
                                     ] ;
                     
                     rdfs:seeAlso "http://www.omgsysml.org/qudv#Quantity" ;
                     
                     rdfs:comment """A DerivedQuantityKind is a QuantityKind that represents a kind of quantity that is defined as a product of powers of one or
more other kinds of quantity. A DerivedQuantityKind may also be used to define a synonym kind of quantity for another kind
of quantity.
For example \"velocity\" can be specified as the product of \"length\" to the power one times \"time\" to the power minus one, and
subsequently \"speed\" can be specified as \"velocity\" to the power one.""" ;
                     
                     rdfs:isDefinedBy "http://purl.oclc.org/NET/ssnx/qu" ;
                     
                     dc:source "skos:exactMatch 'DerivedQuantityKind ' [SysML 1.2-QUDV] http://www.omgwiki.org/OMGSysML/doku.php?id=sysml-qudv:quantities_units_dimensions_values_qudv" .



###  http://purl.oclc.org/NET/ssnx/qu/qu#DerivedUnit

:DerivedUnit rdf:type owl:Class ;
             
             rdfs:label "DerivedUnit" ;
             
             rdfs:subClassOf :Unit ,
                             [ rdf:type owl:Restriction ;
                               owl:onProperty :unitFactor ;
                               owl:someValuesFrom :UnitFactor
                             ] ;
             
             rdfs:seeAlso "http://www.omgsysml.org/qudv#Unit" ;
             
             rdfs:comment """A DerivedUnit is a Unit that represents a measurement unit that is defined as a product of powers of one or more other
measurement units.
For example the measurement unit \"metre per second\" for \"velocity\" is specified as the product of \"metre\" to the power one
times \"second\" to the power minus one""" ;
             
             rdfs:isDefinedBy "http://purl.oclc.org/NET/ssnx/qu" ;
             
             dc:source "skos:exactMatch 'DerivedUnit' [SysML 1.2-QUDV] http://www.omgwiki.org/OMGSysML/doku.php?id=sysml-qudv:quantities_units_dimensions_values_qudv" .



###  http://purl.oclc.org/NET/ssnx/qu/qu#Dimension

:Dimension rdf:type owl:Class ;
           
           rdfs:label "Dimension" ;
           
           rdfs:subClassOf [ rdf:type owl:Class ;
                             owl:intersectionOf ( [ rdf:type owl:Restriction ;
                                                    owl:onProperty :dimensionFactor ;
                                                    owl:allValuesFrom :DimensionFactor
                                                  ]
                                                  [ rdf:type owl:Restriction ;
                                                    owl:onProperty :symbolicExpression ;
                                                    owl:qualifiedCardinality "1"^^xsd:nonNegativeInteger ;
                                                    owl:onDataRange xsd:string
                                                  ]
                                                )
                           ] ;
           
           rdfs:comment """A Dimension represents the [VIM] concept of 'quantity dimension' that is defined as 'expression of the dependence of a quantity on the base quantities of a system of quantities as a product of powers of factors corresponding to the base quantities, omitting any numerical factor.'

For example in the ISQ the quantity dimension of 'force' is denoted by dim F = Lï¿½Mï¿½T^2, where 'F' is the symbol for 'force', and 'L', 'M', 'T' are the symbols for the ISQ base quantities 'length', 'mass' and 'time' respectively.

The Dimension of any QuantityKind can be derived through the algorithm that is defined in C.5.3.20 with SystemOfQuantities. The actual Dimension for a given QuantityKind depends on the choice of baseQuantityKind specified in a SystemOfQuantities.""" ;
           
           rdfs:isDefinedBy "http://purl.oclc.org/NET/ssnx/qu" ;
           
           dc:source "skos:exactMatch 'Dimension' [SysML 1.2-QUDV] http://www.omgwiki.org/OMGSysML/doku.php?id=sysml-qudv:quantities_units_dimensions_values_qudv" ;
           
           rdfs:seeAlso "http://www.omgsysml.org/qudv#Dimension" .



###  http://purl.oclc.org/NET/ssnx/qu/qu#DimensionFactor

:DimensionFactor rdf:type owl:Class ;
                 
                 rdfs:label "DimensionFactor" ;
                 
                 rdfs:subClassOf [ rdf:type owl:Restriction ;
                                   owl:onProperty :baseDimension ;
                                   owl:onClass :QuantityKind ;
                                   owl:qualifiedCardinality "1"^^xsd:nonNegativeInteger
                                 ] ;
                 
                 dc:source "skos:exactMatch 'DimensionFactor' [SysML 1.2-QUDV] http://www.omgwiki.org/OMGSysML/doku.php?id=sysml-qudv:quantities_units_dimensions_values_qudv" ;
                 
                 rdfs:isDefinedBy "http://purl.oclc.org/NET/ssnx/qu" ;
                 
                 rdfs:comment "A DimensionFactor represents a factor in the product of powers that defines a Dimension." ;
                 
                 rdfs:seeAlso "http://www.omgsysml.org/qudv#Dimension" .



###  http://purl.oclc.org/NET/ssnx/qu/qu#GeneralConversionUnit

:GeneralConversionUnit rdf:type owl:Class ;
                       
                       rdfs:label "GeneralConversionUnit" ;
                       
                       rdfs:subClassOf :ConversionBasedUnit ,
                                       [ rdf:type owl:Restriction ;
                                         owl:onProperty :expression ;
                                         owl:qualifiedCardinality "1"^^xsd:nonNegativeInteger ;
                                         owl:onDataRange xsd:string
                                       ] ;
                       
                       rdfs:comment """A GeneralConversionUnit is a ConversionBasedUnit that represents a measurement unit that is defined with respect to another
reference measurement unit through a conversion relationship expressed in some syntax through a general mathematical
expression.
The unit conversion relationship is defined by the following equation:
valueRU / valueCU = f(valueRU, valueCU)
where:
valueRU is the quantity value expressed in the referenceUnit, and,
valueCU is the quantity value expressed in the GeneralConversionUnit, and,
f(valueRU, valueCU) is a mathematical expression that includes valueRU and valueCU.""" ;
                       
                       rdfs:isDefinedBy "http://purl.oclc.org/NET/ssnx/qu" ;
                       
                       rdfs:seeAlso "http://www.omgsysml.org/qudv#Unit" ;
                       
                       dc:source "skos:exactMatch 'GeneralConversionUnit' [SysML 1.2-QUDV] http://www.omgwiki.org/OMGSysML/doku.php?id=sysml-qudv:quantities_units_dimensions_values_qudv" .



###  http://purl.oclc.org/NET/ssnx/qu/qu#LinearConversionUnit

:LinearConversionUnit rdf:type owl:Class ;
                      
                      rdfs:label "LinearConversionUnit" ;
                      
                      rdfs:subClassOf :ConversionBasedUnit ,
                                      [ rdf:type owl:Restriction ;
                                        owl:onProperty :conversionFactor ;
                                        owl:qualifiedCardinality "1"^^xsd:nonNegativeInteger ;
                                        owl:onDataRange xsd:double
                                      ] ;
                      
                      rdfs:seeAlso "http://www.omgsysml.org/qudv#Unit" ;
                      
                      rdfs:comment """A LinearConversionUnit is a ConversionBasedUnit that represents a measurement unit that is defined with respect to another
measurement reference unit through a linear conversion relationship with a conversion factor.
The unit conversion relationship is defined by the following equation:
valueRU = factor · valueCU,
where:
valueRU is the quantity value expressed in the referenceUnit, and,
valueCU is the quantity value expressed in the LinearConversionUnit.""" ;
                      
                      rdfs:isDefinedBy "http://purl.oclc.org/NET/ssnx/qu" ;
                      
                      dc:source "skos:exactMatch 'LinearConversionUnit' [SysML 1.2-QUDV] http://www.omgwiki.org/OMGSysML/doku.php?id=sysml-qudv:quantities_units_dimensions_values_qudv" .



###  http://purl.oclc.org/NET/ssnx/qu/qu#Prefix

:Prefix rdf:type owl:Class ;
        
        rdfs:label "Prefix" ;
        
        rdfs:subClassOf [ rdf:type owl:Class ;
                          owl:intersectionOf ( [ rdf:type owl:Restriction ;
                                                 owl:onProperty :name ;
                                                 owl:qualifiedCardinality "1"^^xsd:nonNegativeInteger ;
                                                 owl:onDataRange xsd:string
                                               ]
                                               [ rdf:type owl:Restriction ;
                                                 owl:onProperty :symbol ;
                                                 owl:qualifiedCardinality "1"^^xsd:nonNegativeInteger ;
                                                 owl:onDataRange xsd:string
                                               ]
                                               [ rdf:type owl:Restriction ;
                                                 owl:onProperty :unitMultipleFactor ;
                                                 owl:qualifiedCardinality "1"^^xsd:nonNegativeInteger ;
                                                 owl:onDataRange xsd:double
                                               ]
                                             )
                        ] ;
        
        dc:source "skos:exactMatch 'Prefix' [SysML 1.2-QUDV] http://www.omgwiki.org/OMGSysML/doku.php?id=sysml-qudv:quantities_units_dimensions_values_qudv" ;
        
        rdfs:comment """A Prefix represents a named multiple or submultiple multiplication factor used in the specification of a PrefixedUnit. A
SystemOfUnits may specify a set of prefixes.""" ;
        
        rdfs:isDefinedBy "http://purl.oclc.org/NET/ssnx/qu" ;
        
        rdfs:seeAlso "http://www.omgsysml.org/qudv#Unit" .



###  http://purl.oclc.org/NET/ssnx/qu/qu#PrefixedUnit

:PrefixedUnit rdf:type owl:Class ;
              
              rdfs:label "PrefixedUnit" ;
              
              rdfs:subClassOf :ConversionBasedUnit ,
                              [ rdf:type owl:Restriction ;
                                owl:onProperty :prefix ;
                                owl:onClass :Prefix ;
                                owl:qualifiedCardinality "1"^^xsd:nonNegativeInteger
                              ] ;
              
              rdfs:isDefinedBy "http://purl.oclc.org/NET/ssnx/qu" ;
              
              rdfs:comment """A Prefix represents a named multiple or submultiple multiplication factor used in the specification of a PrefixedUnit. A
SystemOfUnits may specify a set of prefixes.""" ;
              
              rdfs:seeAlso "http://www.omgsysml.org/qudv#Unit" ;
              
              dc:source "skos:exactMatch 'Prefix' [SysML 1.2-QUDV] http://www.omgwiki.org/OMGSysML/doku.php?id=sysml-qudv:quantities_units_dimensions_values_qudv" .



###  http://purl.oclc.org/NET/ssnx/qu/qu#PropertyKind

:PropertyKind rdf:type owl:Class ;
              
              rdfs:label "PropertyKind " ;
              
              rdfs:seeAlso "http://www.omgsysml.org/qudv#Quantity" ;
              
              rdfs:comment "A PropertyKind  is a meta-property which helps to characterise categories of properties e.g. scalar, vector" ;
              
              rdfs:isDefinedBy "http://purl.oclc.org/NET/ssnx/qu" .



###  http://purl.oclc.org/NET/ssnx/qu/qu#QuantityKind

:QuantityKind rdf:type owl:Class ;
              
              rdfs:label "QuantityKind" ;
              
              rdfs:subClassOf [ rdf:type owl:Class ;
                                owl:intersectionOf ( [ rdf:type owl:Restriction ;
                                                       owl:onProperty :scale ;
                                                       owl:onClass :Scale ;
                                                       owl:maxQualifiedCardinality "1"^^xsd:nonNegativeInteger
                                                     ]
                                                     [ rdf:type owl:Restriction ;
                                                       owl:onProperty :name ;
                                                       owl:qualifiedCardinality "1"^^xsd:nonNegativeInteger ;
                                                       owl:onDataRange xsd:string
                                                     ]
                                                     [ rdf:type owl:Restriction ;
                                                       owl:onProperty :symbol ;
                                                       owl:qualifiedCardinality "1"^^xsd:nonNegativeInteger ;
                                                       owl:onDataRange xsd:string
                                                     ]
                                                     [ rdf:type owl:Restriction ;
                                                       owl:onProperty :definitionURI ;
                                                       owl:maxQualifiedCardinality "1"^^xsd:nonNegativeInteger ;
                                                       owl:onDataRange xsd:string
                                                     ]
                                                     [ rdf:type owl:Restriction ;
                                                       owl:onProperty :description ;
                                                       owl:maxQualifiedCardinality "1"^^xsd:nonNegativeInteger ;
                                                       owl:onDataRange xsd:string
                                                     ]
                                                   )
                              ] ;
              
              rdfs:seeAlso "http://www.omgsysml.org/qudv#Quantity" ;
              
              rdfs:comment """A QuantityKind is an abstract classifier that represents the [VIM] concept of \"kind of quantity\" that is defined as \"aspect
common to mutually comparable quantities.\" A QuantityKind represents the essence of a quantity without any numerical
value or unit. Quantities of the same kind within a given system of quantities have the same quantity dimension. However,
quantities of the same dimension are not necessarily of the same kind.""" ;
              
              dc:source "skos:exactMatch 'QuantityKind' [SysML 1.2-QUDV] http://www.omgwiki.org/OMGSysML/doku.php?id=sysml-qudv:quantities_units_dimensions_values_qudv" ;
              
              rdfs:isDefinedBy "http://purl.oclc.org/NET/ssnx/qu" .



###  http://purl.oclc.org/NET/ssnx/qu/qu#QuantityKindFactor

:QuantityKindFactor rdf:type owl:Class ;
                    
                    rdfs:label "QuantityKindFactor" ;
                    
                    rdfs:subClassOf [ rdf:type owl:Class ;
                                      owl:intersectionOf ( [ rdf:type owl:Restriction ;
                                                             owl:onProperty :factorQuantityKind ;
                                                             owl:onClass :QuantityKind ;
                                                             owl:qualifiedCardinality "1"^^xsd:nonNegativeInteger
                                                           ]
                                                           [ rdf:type owl:Restriction ;
                                                             owl:onProperty :exponent ;
                                                             owl:qualifiedCardinality "1"^^xsd:nonNegativeInteger ;
                                                             owl:onDataRange xsd:double
                                                           ]
                                                         )
                                    ] ;
                    
                    rdfs:seeAlso "http://www.omgsysml.org/qudv#Quantity" ;
                    
                    rdfs:comment "A QuantityKindFactor represents a factor in the product of powers that defines a DerivedQuantityKind." ;
                    
                    dc:source "skos:exactMatch 'QuantityKindFactor' [SysML 1.2-QUDV] http://www.omgwiki.org/OMGSysML/doku.php?id=sysml-qudv:quantities_units_dimensions_values_qudv" ;
                    
                    rdfs:isDefinedBy "http://purl.oclc.org/NET/ssnx/qu" .



###  http://purl.oclc.org/NET/ssnx/qu/qu#Scale

:Scale rdf:type owl:Class ;
       
       rdfs:label "Scale" ;
       
       rdfs:subClassOf [ rdf:type owl:Class ;
                         owl:intersectionOf ( [ rdf:type owl:Restriction ;
                                                owl:onProperty :scaleValueDefinition ;
                                                owl:someValuesFrom :ScaleValueDefinition
                                              ]
                                              [ rdf:type owl:Restriction ;
                                                owl:onProperty :unit ;
                                                owl:onClass :Unit ;
                                                owl:maxQualifiedCardinality "1"^^xsd:nonNegativeInteger
                                              ]
                                            )
                       ] ;
       
       rdfs:seeAlso "http://www.omgsysml.org/qudv#Scale" ;
       
       dc:source "skos:exactMatch 'Scale' [SysML 1.2-QUDV] http://www.omgwiki.org/OMGSysML/doku.php?id=sysml-qudv:quantities_units_dimensions_values_qudv" ;
       
       rdfs:comment """A Scale represents the [VIM] concept of a \"measurement scale\" that is defined as an \"ordered set of quantity values of
quantities of a given kind of quantity used in ranking, according to magnitude, quantities of that kind.\" A Scale specifies one
or more fixed values that have a specific significance in the definition of the associating QuantityKind.
For example the \"thermodynamic temperature\" kind of quantity is defined by specifying the values of 0 and 273.16 kelvin as
the temperatures of absolute zero and the triple point of water respectively.
A Scale does not always need to specify a unit. For example the \"Rockwell C Hardness Scale\" or the \"Beaufort Wind Force
Scale\" are ordinal scales that do not have a particular associated unit. Similarly, subjective scales for a \"priority\" or \"risk\" kind
of quantity with e.g. value definitions 0 for \"low\", 1 for \"medium\" and 3 for \"high\" do not have a particular associated unit.""" ;
       
       rdfs:isDefinedBy "http://purl.oclc.org/NET/ssnx/qu" .



###  http://purl.oclc.org/NET/ssnx/qu/qu#ScaleValueDefinition

:ScaleValueDefinition rdf:type owl:Class ;
                      
                      rdfs:label "ScaleValueDefinition" ;
                      
                      rdfs:subClassOf [ rdf:type owl:Class ;
                                        owl:intersectionOf ( [ rdf:type owl:Restriction ;
                                                               owl:onProperty :description ;
                                                               owl:qualifiedCardinality "1"^^xsd:nonNegativeInteger ;
                                                               owl:onDataRange xsd:string
                                                             ]
                                                             [ rdf:type owl:Restriction ;
                                                               owl:onProperty :numericalValue ;
                                                               owl:qualifiedCardinality "1"^^xsd:nonNegativeInteger ;
                                                               owl:onDataRange xsd:double
                                                             ]
                                                           )
                                      ] ;
                      
                      rdfs:comment "A ScaleValueDefinition represents a specific value for a measurement scale." ;
                      
                      rdfs:seeAlso "http://www.omgsysml.org/qudv#Scale" ;
                      
                      dc:source "skos:exactMatch 'ScaleValueDefinition' [SysML 1.2-QUDV] http://www.omgwiki.org/OMGSysML/doku.php?id=sysml-qudv:quantities_units_dimensions_values_qudv" ;
                      
                      rdfs:isDefinedBy "http://purl.oclc.org/NET/ssnx/qu" .



###  http://purl.oclc.org/NET/ssnx/qu/qu#SimpleQuantityKind

:SimpleQuantityKind rdf:type owl:Class ;
                    
                    rdfs:label "SimpleQuantityKind" ;
                    
                    rdfs:subClassOf :QuantityKind ;
                    
                    rdfs:comment """A SimpleQuantityKind is a QuantityKind that represents a kind of quantity that does not depend on any other QuantityKind.
Typically a base quantity would be specified as a SimpleQuantityKind.""" ;
                    
                    dc:source "skos:exactMatch 'SimpleQuantityKind' [SysML 1.2-QUDV] http://www.omgwiki.org/OMGSysML/doku.php?id=sysml-qudv:quantities_units_dimensions_values_qudv" ;
                    
                    rdfs:isDefinedBy "http://purl.oclc.org/NET/ssnx/qu" ;
                    
                    rdfs:seeAlso "http://www.omgsysml.org/qudv#Quantity" .



###  http://purl.oclc.org/NET/ssnx/qu/qu#SimpleUnit

:SimpleUnit rdf:type owl:Class ;
            
            rdfs:label "SimpleUnit" ;
            
            rdfs:subClassOf :Unit ;
            
            rdfs:seeAlso "http://www.omgsysml.org/qudv#Unit" ;
            
            rdfs:comment """A SimpleUnit is a Unit that represents a measurement unit that does not depend on any other Unit. Typically a base unit would
be specified as a SimpleUnit.""" ;
            
            dc:source "skos:exactMatch 'SimpleUnit' [SysML 1.2-QUDV] http://www.omgwiki.org/OMGSysML/doku.php?id=sysml-qudv:quantities_units_dimensions_values_qudv" ;
            
            rdfs:isDefinedBy "http://purl.oclc.org/NET/ssnx/qu" .



###  http://purl.oclc.org/NET/ssnx/qu/qu#SpecializedQuantityKind

:SpecializedQuantityKind rdf:type owl:Class ;
                         
                         rdfs:label "SpecializedQuantityKind" ;
                         
                         rdfs:subClassOf :QuantityKind ,
                                         [ rdf:type owl:Restriction ;
                                           owl:onProperty :generalQuantityKind ;
                                           owl:onClass :QuantityKind ;
                                           owl:qualifiedCardinality "1"^^xsd:nonNegativeInteger
                                         ] ;
                         
                         rdfs:isDefinedBy "http://purl.oclc.org/NET/ssnx/qu" ;
                         
                         rdfs:seeAlso "http://www.omgsysml.org/qudv#Quantity" ;
                         
                         rdfs:comment """A SpecializedQuantityKind is a QuantityKind that represents a kind of quantity that is a specialization of another kind of
quantity.
For example, \"distance\", \"width\", \"depth\", \"radius\" and \"wavelength\" can all be specified as specializations of the \"length\"
SimpleQuantityKind.""" ;
                         
                         dc:source "skos:exactMatch 'SpecializedQuantityKind' [SysML 1.2-QUDV] http://www.omgwiki.org/OMGSysML/doku.php?id=sysml-qudv:quantities_units_dimensions_values_qudv" .



###  http://purl.oclc.org/NET/ssnx/qu/qu#SystemOfQuantities

:SystemOfQuantities rdf:type owl:Class ;
                    
                    rdfs:label "SystemOfQuantities" ;
                    
                    rdfs:subClassOf [ rdf:type owl:Class ;
                                      owl:intersectionOf ( [ rdf:type owl:Restriction ;
                                                             owl:onProperty :dimension ;
                                                             owl:someValuesFrom :Dimension
                                                           ]
                                                           [ rdf:type owl:Restriction ;
                                                             owl:onProperty :quantityComponent ;
                                                             owl:someValuesFrom :QuantityKind
                                                           ]
                                                           [ rdf:type owl:Restriction ;
                                                             owl:onProperty :baseQuantityKind ;
                                                             owl:allValuesFrom :QuantityKind
                                                           ]
                                                           [ rdf:type owl:Restriction ;
                                                             owl:onProperty :name ;
                                                             owl:qualifiedCardinality "1"^^xsd:nonNegativeInteger ;
                                                             owl:onDataRange xsd:string
                                                           ]
                                                           [ rdf:type owl:Restriction ;
                                                             owl:onProperty :symbol ;
                                                             owl:qualifiedCardinality "1"^^xsd:nonNegativeInteger ;
                                                             owl:onDataRange xsd:string
                                                           ]
                                                           [ rdf:type owl:Restriction ;
                                                             owl:onProperty :definitionURI ;
                                                             owl:maxQualifiedCardinality "1"^^xsd:nonNegativeInteger ;
                                                             owl:onDataRange xsd:string
                                                           ]
                                                           [ rdf:type owl:Restriction ;
                                                             owl:onProperty :description ;
                                                             owl:maxQualifiedCardinality "1"^^xsd:nonNegativeInteger ;
                                                             owl:onDataRange xsd:string
                                                           ]
                                                         )
                                    ] ;
                    
                    rdfs:seeAlso "http://www.omgsysml.org/qudv#Dimension" ;
                    
                    rdfs:isDefinedBy "http://purl.oclc.org/NET/ssnx/qu" ;
                    
                    rdfs:comment """A SystemOfQuantities represents the [VIM] concept of 'system of quantities' that is defined as a 'set of quantities together with a set of non-contradictory equations relating those quantities'. It collects a list of QuantityKind that specifies the kinds of quantity that are known in the system.

The International System of Quantities (ISQ) is an example of a SystemOfQuantities, defined in ISO 31 and ISO/IEC 80000.""" ;
                    
                    dc:source "skos:exactMatch 'SystemOfQuantities' [SysML 1.2-QUDV] http://www.omgwiki.org/OMGSysML/doku.php?id=sysml-qudv:quantities_units_dimensions_values_qudv" .



###  http://purl.oclc.org/NET/ssnx/qu/qu#SystemOfUnits

:SystemOfUnits rdf:type owl:Class ;
               
               rdfs:label "SystemOfUnits" ;
               
               rdfs:subClassOf [ rdf:type owl:Class ;
                                 owl:intersectionOf ( [ rdf:type owl:Restriction ;
                                                        owl:onProperty :unitComponent ;
                                                        owl:someValuesFrom :Unit
                                                      ]
                                                      [ rdf:type owl:Restriction ;
                                                        owl:onProperty :baseUnit ;
                                                        owl:allValuesFrom :Unit
                                                      ]
                                                      [ rdf:type owl:Restriction ;
                                                        owl:onProperty :prefix ;
                                                        owl:allValuesFrom :Prefix
                                                      ]
                                                      [ rdf:type owl:Restriction ;
                                                        owl:onProperty :systemOfQuantities ;
                                                        owl:allValuesFrom :SystemOfQuantities
                                                      ]
                                                      [ rdf:type owl:Restriction ;
                                                        owl:onProperty :name ;
                                                        owl:qualifiedCardinality "1"^^xsd:nonNegativeInteger ;
                                                        owl:onDataRange xsd:string
                                                      ]
                                                      [ rdf:type owl:Restriction ;
                                                        owl:onProperty :symbol ;
                                                        owl:qualifiedCardinality "1"^^xsd:nonNegativeInteger ;
                                                        owl:onDataRange xsd:string
                                                      ]
                                                      [ rdf:type owl:Restriction ;
                                                        owl:onProperty :definitionURI ;
                                                        owl:maxQualifiedCardinality "1"^^xsd:nonNegativeInteger ;
                                                        owl:onDataRange xsd:string
                                                      ]
                                                      [ rdf:type owl:Restriction ;
                                                        owl:onProperty :description ;
                                                        owl:maxQualifiedCardinality "1"^^xsd:nonNegativeInteger ;
                                                        owl:onDataRange xsd:string
                                                      ]
                                                    )
                               ] ;
               
               rdfs:isDefinedBy "http://purl.oclc.org/NET/ssnx/qu" ;
               
               dc:source "skos:exactMatch 'SystemOfUnits' [SysML 1.2-QUDV] http://www.omgwiki.org/OMGSysML/doku.php?id=sysml-qudv:quantities_units_dimensions_values_qudv" ;
               
               rdfs:seeAlso "http://www.omgsysml.org/qudv#Dimension" ;
               
               rdfs:comment "A SystemOfUnits represents the [VIM] concept of 'system of units' that is defined as 'set of base units and derived units, together with their multiples and submultiples, defined in accordance with given rules, for a given system of quantities'. It collects a list of Unit that are known in the system. A SysML SystemOfUnits only optionally defines multiples and submultiples." .



###  http://purl.oclc.org/NET/ssnx/qu/qu#Unit

:Unit rdf:type owl:Class ;
      
      rdfs:label "Unit" ;
      
      rdfs:subClassOf [ rdf:type owl:Class ;
                        owl:intersectionOf ( [ rdf:type owl:Restriction ;
                                               owl:onProperty :quantityKind ;
                                               owl:onClass :QuantityKind ;
                                               owl:maxQualifiedCardinality "1"^^xsd:nonNegativeInteger
                                             ]
                                             [ rdf:type owl:Restriction ;
                                               owl:onProperty :name ;
                                               owl:qualifiedCardinality "1"^^xsd:nonNegativeInteger ;
                                               owl:onDataRange xsd:string
                                             ]
                                             [ rdf:type owl:Restriction ;
                                               owl:onProperty :symbol ;
                                               owl:qualifiedCardinality "1"^^xsd:nonNegativeInteger ;
                                               owl:onDataRange xsd:string
                                             ]
                                             [ rdf:type owl:Restriction ;
                                               owl:onProperty :definitionURI ;
                                               owl:maxQualifiedCardinality "1"^^xsd:nonNegativeInteger ;
                                               owl:onDataRange xsd:string
                                             ]
                                             [ rdf:type owl:Restriction ;
                                               owl:onProperty :description ;
                                               owl:maxQualifiedCardinality "1"^^xsd:nonNegativeInteger ;
                                               owl:onDataRange xsd:string
                                             ]
                                           )
                      ] ;
      
      dc:source "skos:exactMatch 'Unit' [SysML 1.2-QUDV] http://www.omgwiki.org/OMGSysML/doku.php?id=sysml-qudv:quantities_units_dimensions_values_qudv" ;
      
      rdfs:seeAlso "http://www.omgsysml.org/qudv#Unit" ;
      
      rdfs:isDefinedBy "http://purl.oclc.org/NET/ssnx/qu" ;
      
      rdfs:comment """A Unit is an abstract classifier that represents the [VIM] concept of \"measurement unit\" that is defined as \"real scalar quantity,
defined and adopted by convention, with which any other quantity of the same kind can be compared to express the ratio of the
two quantities as a number.\"""" .



###  http://purl.oclc.org/NET/ssnx/qu/qu#UnitFactor

:UnitFactor rdf:type owl:Class ;
            
            rdfs:label "UnitFactor" ;
            
            rdfs:subClassOf [ rdf:type owl:Class ;
                              owl:intersectionOf ( [ rdf:type owl:Restriction ;
                                                     owl:onProperty :unit ;
                                                     owl:onClass :Unit ;
                                                     owl:qualifiedCardinality "1"^^xsd:nonNegativeInteger
                                                   ]
                                                   [ rdf:type owl:Restriction ;
                                                     owl:onProperty :exponent ;
                                                     owl:qualifiedCardinality "1"^^xsd:nonNegativeInteger ;
                                                     owl:onDataRange xsd:double
                                                   ]
                                                 )
                            ] ;
            
            rdfs:seeAlso "http://www.omgsysml.org/qudv#Unit" ;
            
            rdfs:comment "A UnitFactor represents a factor in the product of powers that defines a DerivedUnit." ;
            
            rdfs:isDefinedBy "http://purl.oclc.org/NET/ssnx/qu" ;
            
            dc:source "skos:exactMatch 'UnitFactor' [SysML 1.2-QUDV] http://www.omgwiki.org/OMGSysML/doku.php?id=sysml-qudv:quantities_units_dimensions_values_qudv" .



###  http://www.w3.org/2002/07/owl#Thing

owl:Thing rdf:type owl:Class .





#################################################################
#
#    General axioms
#
#################################################################


[ rdf:type owl:AllDisjointClasses ;
  owl:members ( :QuantityKind
                :QuantityKindFactor
                :Scale
                :ScaleValueDefinition
                :SystemOfQuantities
                :SystemOfUnits
                :Unit
                :UnitFactor
              )
] .




###  Generated by the OWL API (version 3.4.2) http://owlapi.sourceforge.net

