<?xml version="1.0"?>


<!DOCTYPE rdf:RDF [
    <!ENTITY owl "http://www.w3.org/2002/07/owl#" >
    <!ENTITY xsd "http://www.w3.org/2001/XMLSchema#" >
    <!ENTITY rdfs "http://www.w3.org/2000/01/rdf-schema#" >
    <!ENTITY edxl_cap "http://fpc.ufba.br/ontologies/edxl_cap#" >
    <!ENTITY rdf "http://www.w3.org/1999/02/22-rdf-syntax-ns#" >
]>


<rdf:RDF xmlns="http://fpc.ufba.br/ontologies/edxl_cap#"
     xml:base="http://fpc.ufba.br/ontologies/edxl_cap"
     xmlns:rdfs="http://www.w3.org/2000/01/rdf-schema#"
     xmlns:edxl_cap="http://fpc.ufba.br/ontologies/edxl_cap#"
     xmlns:owl="http://www.w3.org/2002/07/owl#"
     xmlns:xsd="http://www.w3.org/2001/XMLSchema#"
     xmlns:rdf="http://www.w3.org/1999/02/22-rdf-syntax-ns#">
    <owl:Ontology rdf:about="http://fpc.ufba.br/ontologies/edxl_cap">
        <rights xml:lang="en">(c) The RESCUER project - http://www.rescuer-project.org/</rights>
        <status xml:lang="en">An ongoing ontology for communication interoperability between systems in the context of the RESCUER Project. This propose is based on EDXL documentation (https://www.oasis-open.org/committees/tc_home.php?wg_abbrev=emergency).</status>
        <contributor xml:lang="en">Lais Salvador (UFBA)</contributor>
        <contributor xml:lang="en">Rebeca Barros (UFBA)</contributor>
        <contributor xml:lang="en">Reinaldo Almeida (UFBA)</contributor>
    </owl:Ontology>
    


    <!-- 
    ///////////////////////////////////////////////////////////////////////////////////////
    //
    // Annotation properties
    //
    ///////////////////////////////////////////////////////////////////////////////////////
     -->

    


    <!-- http://fpc.ufba.br/ontologies/edxl_cap#contributor -->

    <owl:AnnotationProperty rdf:about="&edxl_cap;contributor"/>
    


    <!-- http://fpc.ufba.br/ontologies/edxl_cap#rights -->

    <owl:AnnotationProperty rdf:about="&edxl_cap;rights"/>
    


    <!-- http://fpc.ufba.br/ontologies/edxl_cap#status -->

    <owl:AnnotationProperty rdf:about="&edxl_cap;status"/>
    


    <!-- 
    ///////////////////////////////////////////////////////////////////////////////////////
    //
    // Object Properties
    //
    ///////////////////////////////////////////////////////////////////////////////////////
     -->

    


    <!-- http://fpc.ufba.br/ontologies/edxl_cap#hasArea -->

    <owl:ObjectProperty rdf:about="&edxl_cap;hasArea">
        <rdfs:range rdf:resource="&edxl_cap;Area"/>
        <rdfs:domain rdf:resource="&edxl_cap;Info"/>
        <owl:inverseOf rdf:resource="&edxl_cap;isAreaOf"/>
    </owl:ObjectProperty>
    


    <!-- http://fpc.ufba.br/ontologies/edxl_cap#hasCategory -->

    <owl:ObjectProperty rdf:about="&edxl_cap;hasCategory">
        <rdfs:range rdf:resource="&edxl_cap;Category"/>
        <rdfs:domain rdf:resource="&edxl_cap;Info"/>
    </owl:ObjectProperty>
    


    <!-- http://fpc.ufba.br/ontologies/edxl_cap#hasCertainty -->

    <owl:ObjectProperty rdf:about="&edxl_cap;hasCertainty">
        <rdfs:range rdf:resource="&edxl_cap;Certainty"/>
        <rdfs:domain rdf:resource="&edxl_cap;Info"/>
    </owl:ObjectProperty>
    


    <!-- http://fpc.ufba.br/ontologies/edxl_cap#hasIncidentRelated -->

    <owl:ObjectProperty rdf:about="&edxl_cap;hasIncidentRelated">
        <rdfs:domain rdf:resource="&edxl_cap;AlertMessage"/>
        <rdfs:range rdf:resource="&edxl_cap;Incident"/>
    </owl:ObjectProperty>
    


    <!-- http://fpc.ufba.br/ontologies/edxl_cap#hasInfo -->

    <owl:ObjectProperty rdf:about="&edxl_cap;hasInfo">
        <rdfs:domain rdf:resource="&edxl_cap;AlertMessage"/>
        <rdfs:range rdf:resource="&edxl_cap;Info"/>
    </owl:ObjectProperty>
    


    <!-- http://fpc.ufba.br/ontologies/edxl_cap#hasMsgType -->

    <owl:ObjectProperty rdf:about="&edxl_cap;hasMsgType">
        <rdfs:domain rdf:resource="&edxl_cap;AlertMessage"/>
        <rdfs:range rdf:resource="&edxl_cap;MsgType"/>
    </owl:ObjectProperty>
    


    <!-- http://fpc.ufba.br/ontologies/edxl_cap#hasReferences -->

    <owl:ObjectProperty rdf:about="&edxl_cap;hasReferences">
        <rdfs:comment xml:lang="en">identifying earlier message(s) referenced by the alert message</rdfs:comment>
        <rdfs:domain rdf:resource="&edxl_cap;AlertMessage"/>
        <rdfs:range rdf:resource="&edxl_cap;AlertMessage"/>
        <owl:inverseOf rdf:resource="&edxl_cap;isReferencedBy"/>
    </owl:ObjectProperty>
    


    <!-- http://fpc.ufba.br/ontologies/edxl_cap#hasResource -->

    <owl:ObjectProperty rdf:about="&edxl_cap;hasResource">
        <rdfs:domain rdf:resource="&edxl_cap;Info"/>
        <rdfs:range rdf:resource="&edxl_cap;Resource"/>
        <owl:inverseOf rdf:resource="&edxl_cap;isResourceOf"/>
    </owl:ObjectProperty>
    


    <!-- http://fpc.ufba.br/ontologies/edxl_cap#hasResponseType -->

    <owl:ObjectProperty rdf:about="&edxl_cap;hasResponseType">
        <rdfs:domain rdf:resource="&edxl_cap;Info"/>
        <rdfs:range rdf:resource="&edxl_cap;ResponseType"/>
    </owl:ObjectProperty>
    


    <!-- http://fpc.ufba.br/ontologies/edxl_cap#hasScope -->

    <owl:ObjectProperty rdf:about="&edxl_cap;hasScope">
        <rdf:type rdf:resource="&owl;FunctionalProperty"/>
        <rdfs:domain rdf:resource="&edxl_cap;AlertMessage"/>
        <rdfs:range rdf:resource="&edxl_cap;Scope"/>
        <owl:inverseOf rdf:resource="&edxl_cap;isScopeOf"/>
    </owl:ObjectProperty>
    


    <!-- http://fpc.ufba.br/ontologies/edxl_cap#hasSender -->

    <owl:ObjectProperty rdf:about="&edxl_cap;hasSender">
        <rdfs:range rdf:resource="&edxl_cap;Sender"/>
    </owl:ObjectProperty>
    


    <!-- http://fpc.ufba.br/ontologies/edxl_cap#hasSeverity -->

    <owl:ObjectProperty rdf:about="&edxl_cap;hasSeverity">
        <rdfs:domain rdf:resource="&edxl_cap;Info"/>
        <rdfs:range rdf:resource="&edxl_cap;Severity"/>
    </owl:ObjectProperty>
    


    <!-- http://fpc.ufba.br/ontologies/edxl_cap#hasStatus -->

    <owl:ObjectProperty rdf:about="&edxl_cap;hasStatus">
        <rdf:type rdf:resource="&owl;FunctionalProperty"/>
        <rdfs:domain rdf:resource="&edxl_cap;AlertMessage"/>
        <rdfs:range rdf:resource="&edxl_cap;Status"/>
    </owl:ObjectProperty>
    


    <!-- http://fpc.ufba.br/ontologies/edxl_cap#hasUrgency -->

    <owl:ObjectProperty rdf:about="&edxl_cap;hasUrgency">
        <rdfs:domain rdf:resource="&edxl_cap;Info"/>
        <rdfs:range rdf:resource="&edxl_cap;Urgency"/>
    </owl:ObjectProperty>
    


    <!-- http://fpc.ufba.br/ontologies/edxl_cap#isAreaOf -->

    <owl:ObjectProperty rdf:about="&edxl_cap;isAreaOf"/>
    


    <!-- http://fpc.ufba.br/ontologies/edxl_cap#isCategoryOf -->

    <owl:ObjectProperty rdf:about="&edxl_cap;isCategoryOf">
        <owl:inverseOf rdf:resource="&edxl_cap;hasCategory"/>
    </owl:ObjectProperty>
    


    <!-- http://fpc.ufba.br/ontologies/edxl_cap#isCertaintyOf -->

    <owl:ObjectProperty rdf:about="&edxl_cap;isCertaintyOf">
        <owl:inverseOf rdf:resource="&edxl_cap;hasCertainty"/>
    </owl:ObjectProperty>
    


    <!-- http://fpc.ufba.br/ontologies/edxl_cap#isIncidentRelatedTo -->

    <owl:ObjectProperty rdf:about="&edxl_cap;isIncidentRelatedTo">
        <owl:inverseOf rdf:resource="&edxl_cap;hasIncidentRelated"/>
    </owl:ObjectProperty>
    


    <!-- http://fpc.ufba.br/ontologies/edxl_cap#isInfoOf -->

    <owl:ObjectProperty rdf:about="&edxl_cap;isInfoOf">
        <owl:inverseOf rdf:resource="&edxl_cap;hasInfo"/>
    </owl:ObjectProperty>
    


    <!-- http://fpc.ufba.br/ontologies/edxl_cap#isMsgTypeOf -->

    <owl:ObjectProperty rdf:about="&edxl_cap;isMsgTypeOf">
        <owl:inverseOf rdf:resource="&edxl_cap;hasMsgType"/>
    </owl:ObjectProperty>
    


    <!-- http://fpc.ufba.br/ontologies/edxl_cap#isReferencedBy -->

    <owl:ObjectProperty rdf:about="&edxl_cap;isReferencedBy"/>
    


    <!-- http://fpc.ufba.br/ontologies/edxl_cap#isResourceOf -->

    <owl:ObjectProperty rdf:about="&edxl_cap;isResourceOf"/>
    


    <!-- http://fpc.ufba.br/ontologies/edxl_cap#isResponseTypeOf -->

    <owl:ObjectProperty rdf:about="&edxl_cap;isResponseTypeOf">
        <owl:inverseOf rdf:resource="&edxl_cap;hasResponseType"/>
    </owl:ObjectProperty>
    


    <!-- http://fpc.ufba.br/ontologies/edxl_cap#isScopeOf -->

    <owl:ObjectProperty rdf:about="&edxl_cap;isScopeOf">
        <rdf:type rdf:resource="&owl;InverseFunctionalProperty"/>
    </owl:ObjectProperty>
    


    <!-- http://fpc.ufba.br/ontologies/edxl_cap#isSenderOf -->

    <owl:ObjectProperty rdf:about="&edxl_cap;isSenderOf">
        <owl:inverseOf rdf:resource="&edxl_cap;hasSender"/>
    </owl:ObjectProperty>
    


    <!-- http://fpc.ufba.br/ontologies/edxl_cap#isSeverityOf -->

    <owl:ObjectProperty rdf:about="&edxl_cap;isSeverityOf">
        <owl:inverseOf rdf:resource="&edxl_cap;hasSeverity"/>
    </owl:ObjectProperty>
    


    <!-- http://fpc.ufba.br/ontologies/edxl_cap#isStatusOf -->

    <owl:ObjectProperty rdf:about="&edxl_cap;isStatusOf">
        <owl:inverseOf rdf:resource="&edxl_cap;hasStatus"/>
    </owl:ObjectProperty>
    


    <!-- http://fpc.ufba.br/ontologies/edxl_cap#isUrgencyOf -->

    <owl:ObjectProperty rdf:about="&edxl_cap;isUrgencyOf">
        <owl:inverseOf rdf:resource="&edxl_cap;hasUrgency"/>
    </owl:ObjectProperty>
    


    <!-- 
    ///////////////////////////////////////////////////////////////////////////////////////
    //
    // Data properties
    //
    ///////////////////////////////////////////////////////////////////////////////////////
     -->

    


    <!-- http://fpc.ufba.br/ontologies/edxl_cap#addresses -->

    <owl:DatatypeProperty rdf:about="&edxl_cap;addresses">
        <rdfs:comment xml:lang="en">The group listing of intended recipients of the alert message</rdfs:comment>
        <rdfs:domain rdf:resource="&edxl_cap;Scope"/>
        <rdfs:range rdf:resource="&xsd;string"/>
    </owl:DatatypeProperty>
    


    <!-- http://fpc.ufba.br/ontologies/edxl_cap#areaAltitude -->

    <owl:DatatypeProperty rdf:about="&edxl_cap;areaAltitude">
        <rdfs:comment xml:lang="en">The specific or minimum altitude of the affected area of the alert message</rdfs:comment>
        <rdfs:domain rdf:resource="&edxl_cap;Area"/>
        <rdfs:range rdf:resource="&xsd;string"/>
    </owl:DatatypeProperty>
    


    <!-- http://fpc.ufba.br/ontologies/edxl_cap#areaCeiling -->

    <owl:DatatypeProperty rdf:about="&edxl_cap;areaCeiling">
        <rdfs:comment xml:lang="en">The maximum altitude of the affected area of the alert message</rdfs:comment>
        <rdfs:domain rdf:resource="&edxl_cap;Area"/>
        <rdfs:range rdf:resource="&xsd;string"/>
    </owl:DatatypeProperty>
    


    <!-- http://fpc.ufba.br/ontologies/edxl_cap#areaDesc -->

    <owl:DatatypeProperty rdf:about="&edxl_cap;areaDesc">
        <rdfs:comment xml:lang="en">The text describing the affected area of the alert message</rdfs:comment>
        <rdfs:domain rdf:resource="&edxl_cap;Area"/>
        <rdfs:range rdf:resource="&xsd;string"/>
    </owl:DatatypeProperty>
    


    <!-- http://fpc.ufba.br/ontologies/edxl_cap#areaGeoCode -->

    <owl:DatatypeProperty rdf:about="&edxl_cap;areaGeoCode">
        <rdfs:comment xml:lang="en">The geographic code delineating the affected area of the alert message</rdfs:comment>
        <rdfs:domain rdf:resource="&edxl_cap;Area"/>
        <rdfs:range rdf:resource="&xsd;string"/>
    </owl:DatatypeProperty>
    


    <!-- http://fpc.ufba.br/ontologies/edxl_cap#audience -->

    <owl:DatatypeProperty rdf:about="&edxl_cap;audience">
        <rdfs:comment xml:lang="en">The text describing the intended audience of the alert message.</rdfs:comment>
        <rdfs:domain rdf:resource="&edxl_cap;Info"/>
        <rdfs:range rdf:resource="&xsd;string"/>
    </owl:DatatypeProperty>
    


    <!-- http://fpc.ufba.br/ontologies/edxl_cap#certainty -->

    <owl:DatatypeProperty rdf:about="&edxl_cap;certainty">
        <rdfs:comment xml:lang="en">The code denoting the certainty of the subject event of the alert message</rdfs:comment>
        <rdfs:domain rdf:resource="&edxl_cap;Info"/>
        <rdfs:range rdf:resource="&xsd;string"/>
    </owl:DatatypeProperty>
    


    <!-- http://fpc.ufba.br/ontologies/edxl_cap#code -->

    <owl:DatatypeProperty rdf:about="&edxl_cap;code">
        <rdfs:comment xml:lang="en">The code denoting the special handling of the alert message</rdfs:comment>
        <rdfs:domain rdf:resource="&edxl_cap;AlertMessage"/>
        <rdfs:range rdf:resource="&xsd;string"/>
    </owl:DatatypeProperty>
    


    <!-- http://fpc.ufba.br/ontologies/edxl_cap#contact -->

    <owl:DatatypeProperty rdf:about="&edxl_cap;contact">
        <rdfs:comment xml:lang="en">The text describing the contact for follow-up and confirmation of the alert message</rdfs:comment>
        <rdfs:domain rdf:resource="&edxl_cap;Info"/>
        <rdfs:range rdf:resource="&xsd;string"/>
    </owl:DatatypeProperty>
    


    <!-- http://fpc.ufba.br/ontologies/edxl_cap#dateTime -->

    <owl:DatatypeProperty rdf:about="&edxl_cap;dateTime">
        <rdfs:range rdf:resource="&xsd;dateTime"/>
    </owl:DatatypeProperty>
    


    <!-- http://fpc.ufba.br/ontologies/edxl_cap#derefUri -->

    <owl:DatatypeProperty rdf:about="&edxl_cap;derefUri">
        <rdfs:comment xml:lang="en">The base-64 encoded data content of the resource file</rdfs:comment>
        <rdfs:domain rdf:resource="&edxl_cap;Resource"/>
        <rdfs:range rdf:resource="&xsd;string"/>
    </owl:DatatypeProperty>
    


    <!-- http://fpc.ufba.br/ontologies/edxl_cap#description -->

    <owl:DatatypeProperty rdf:about="&edxl_cap;description">
        <rdfs:comment xml:lang="en">The text describing the subject event of the alert message</rdfs:comment>
        <rdfs:domain rdf:resource="&edxl_cap;Info"/>
        <rdfs:range rdf:resource="&xsd;string"/>
    </owl:DatatypeProperty>
    


    <!-- http://fpc.ufba.br/ontologies/edxl_cap#digest -->

    <owl:DatatypeProperty rdf:about="&edxl_cap;digest">
        <rdfs:comment xml:lang="en">The code representing the digital digest (“hash”) computed from the resource file</rdfs:comment>
        <rdfs:domain rdf:resource="&edxl_cap;Resource"/>
        <rdfs:range rdf:resource="&xsd;string"/>
    </owl:DatatypeProperty>
    


    <!-- http://fpc.ufba.br/ontologies/edxl_cap#effective -->

    <owl:DatatypeProperty rdf:about="&edxl_cap;effective">
        <rdfs:comment xml:lang="en">The effective time of the information of the alert message</rdfs:comment>
        <rdfs:domain rdf:resource="&edxl_cap;Info"/>
        <rdfs:subPropertyOf rdf:resource="&edxl_cap;dateTime"/>
        <rdfs:range rdf:resource="&xsd;dateTime"/>
    </owl:DatatypeProperty>
    


    <!-- http://fpc.ufba.br/ontologies/edxl_cap#event -->

    <owl:DatatypeProperty rdf:about="&edxl_cap;event">
        <rdfs:comment xml:lang="en">The text denoting the type of the subject event of the alert message</rdfs:comment>
        <rdfs:domain rdf:resource="&edxl_cap;Info"/>
    </owl:DatatypeProperty>
    


    <!-- http://fpc.ufba.br/ontologies/edxl_cap#eventCode -->

    <owl:DatatypeProperty rdf:about="&edxl_cap;eventCode">
        <rdfs:comment xml:lang="en">A system- specific code identifying the event type of the alert message</rdfs:comment>
        <rdfs:domain rdf:resource="&edxl_cap;Info"/>
    </owl:DatatypeProperty>
    


    <!-- http://fpc.ufba.br/ontologies/edxl_cap#expires -->

    <owl:DatatypeProperty rdf:about="&edxl_cap;expires">
        <rdfs:comment xml:lang="en">The expiry time of the information of the alert message</rdfs:comment>
        <rdfs:domain rdf:resource="&edxl_cap;Info"/>
        <rdfs:subPropertyOf rdf:resource="&edxl_cap;dateTime"/>
        <rdfs:range rdf:resource="&xsd;dateTime"/>
    </owl:DatatypeProperty>
    


    <!-- http://fpc.ufba.br/ontologies/edxl_cap#headline -->

    <owl:DatatypeProperty rdf:about="&edxl_cap;headline">
        <rdfs:comment xml:lang="en">A brief human-readable headline. Note that some displays (for example, short messaging service devices) may only present this headline; it SHOULD be made as direct and actionable as possible while remaining short.</rdfs:comment>
        <rdfs:domain rdf:resource="&edxl_cap;Info"/>
        <rdfs:range rdf:resource="&xsd;string"/>
    </owl:DatatypeProperty>
    


    <!-- http://fpc.ufba.br/ontologies/edxl_cap#identifier -->

    <owl:DatatypeProperty rdf:about="&edxl_cap;identifier">
        <rdfs:comment xml:lang="en">The identifier of the alert message</rdfs:comment>
        <rdfs:domain rdf:resource="&edxl_cap;AlertMessage"/>
        <rdfs:range rdf:resource="&xsd;string"/>
    </owl:DatatypeProperty>
    


    <!-- http://fpc.ufba.br/ontologies/edxl_cap#instruction -->

    <owl:DatatypeProperty rdf:about="&edxl_cap;instruction">
        <rdfs:comment xml:lang="en">The text describing the recommended action to be taken by recipients of the alert message</rdfs:comment>
        <rdfs:domain rdf:resource="&edxl_cap;Info"/>
        <rdfs:range rdf:resource="&xsd;string"/>
    </owl:DatatypeProperty>
    


    <!-- http://fpc.ufba.br/ontologies/edxl_cap#language -->

    <owl:DatatypeProperty rdf:about="&edxl_cap;language">
        <rdfs:comment xml:lang="en">The code denoting the language of the info sub- element of the alert message</rdfs:comment>
        <rdfs:domain rdf:resource="&edxl_cap;Info"/>
        <rdfs:range rdf:resource="&xsd;language"/>
    </owl:DatatypeProperty>
    


    <!-- http://fpc.ufba.br/ontologies/edxl_cap#mimeType -->

    <owl:DatatypeProperty rdf:about="&edxl_cap;mimeType">
        <rdfs:comment xml:lang="en">The identifier of the MIME content type and sub-type describing the resource file</rdfs:comment>
        <rdfs:domain rdf:resource="&edxl_cap;Resource"/>
        <rdfs:range rdf:resource="&xsd;string"/>
    </owl:DatatypeProperty>
    


    <!-- http://fpc.ufba.br/ontologies/edxl_cap#note -->

    <owl:DatatypeProperty rdf:about="&edxl_cap;note">
        <rdfs:comment xml:lang="en">The text describing the purpose or significance of the alert message</rdfs:comment>
        <rdfs:domain>
            <owl:Class>
                <owl:unionOf rdf:parseType="Collection">
                    <rdf:Description rdf:about="&edxl_cap;ErrorType"/>
                    <rdf:Description rdf:about="&edxl_cap;Exercise"/>
                </owl:unionOf>
            </owl:Class>
        </rdfs:domain>
    </owl:DatatypeProperty>
    


    <!-- http://fpc.ufba.br/ontologies/edxl_cap#onset -->

    <owl:DatatypeProperty rdf:about="&edxl_cap;onset">
        <rdfs:comment xml:lang="en">The expected time of the beginning of the subject event of the alert message</rdfs:comment>
        <rdfs:domain rdf:resource="&edxl_cap;Info"/>
        <rdfs:subPropertyOf rdf:resource="&edxl_cap;dateTime"/>
        <rdfs:range rdf:resource="&xsd;dateTime"/>
    </owl:DatatypeProperty>
    


    <!-- http://fpc.ufba.br/ontologies/edxl_cap#parameter -->

    <owl:DatatypeProperty rdf:about="&edxl_cap;parameter">
        <rdfs:comment xml:lang="en">A system- specific additional parameter associated with the alert message</rdfs:comment>
        <rdfs:domain rdf:resource="&edxl_cap;Info"/>
    </owl:DatatypeProperty>
    


    <!-- http://fpc.ufba.br/ontologies/edxl_cap#resourceDesc -->

    <owl:DatatypeProperty rdf:about="&edxl_cap;resourceDesc">
        <rdfs:comment xml:lang="en">The text describing the type and content of the resource file</rdfs:comment>
        <rdfs:domain rdf:resource="&edxl_cap;Resource"/>
        <rdfs:range rdf:resource="&xsd;string"/>
    </owl:DatatypeProperty>
    


    <!-- http://fpc.ufba.br/ontologies/edxl_cap#resourceSize -->

    <owl:DatatypeProperty rdf:about="&edxl_cap;resourceSize">
        <rdfs:comment xml:lang="en">The integer indicating the size of the resource file</rdfs:comment>
        <rdfs:domain rdf:resource="&edxl_cap;Resource"/>
        <rdfs:range rdf:resource="&xsd;string"/>
    </owl:DatatypeProperty>
    


    <!-- http://fpc.ufba.br/ontologies/edxl_cap#resourceURI -->

    <owl:DatatypeProperty rdf:about="&edxl_cap;resourceURI">
        <rdfs:comment xml:lang="en">The identifier of the hyperlink for the resource file</rdfs:comment>
        <rdfs:domain rdf:resource="&edxl_cap;Resource"/>
        <rdfs:range rdf:resource="&xsd;string"/>
    </owl:DatatypeProperty>
    


    <!-- http://fpc.ufba.br/ontologies/edxl_cap#restriction -->

    <owl:DatatypeProperty rdf:about="&edxl_cap;restriction">
        <rdfs:comment xml:lang="en">The text describing the rule for limiting distribution of the restricted alert message</rdfs:comment>
        <rdfs:domain rdf:resource="&edxl_cap;Restricted"/>
        <rdfs:range rdf:resource="&xsd;string"/>
        <rdfs:subPropertyOf rdf:resource="&owl;topDataProperty"/>
    </owl:DatatypeProperty>
    


    <!-- http://fpc.ufba.br/ontologies/edxl_cap#senderName -->

    <owl:DatatypeProperty rdf:about="&edxl_cap;senderName">
        <rdfs:domain rdf:resource="&edxl_cap;Sender"/>
        <rdfs:range rdf:resource="&xsd;string"/>
    </owl:DatatypeProperty>
    


    <!-- http://fpc.ufba.br/ontologies/edxl_cap#sentTime -->

    <owl:DatatypeProperty rdf:about="&edxl_cap;sentTime">
        <rdfs:comment xml:lang="en">The time and date of the origination of the alert message</rdfs:comment>
        <rdfs:domain rdf:resource="&edxl_cap;AlertMessage"/>
        <rdfs:subPropertyOf rdf:resource="&edxl_cap;dateTime"/>
        <rdfs:range rdf:resource="&xsd;dateTime"/>
    </owl:DatatypeProperty>
    


    <!-- http://fpc.ufba.br/ontologies/edxl_cap#source -->

    <owl:DatatypeProperty rdf:about="&edxl_cap;source">
        <rdfs:comment xml:lang="en">The text identifying the source of the alert message</rdfs:comment>
        <rdfs:domain rdf:resource="&edxl_cap;AlertMessage"/>
        <rdfs:range rdf:resource="&xsd;string"/>
    </owl:DatatypeProperty>
    


    <!-- http://fpc.ufba.br/ontologies/edxl_cap#webInfo -->

    <owl:DatatypeProperty rdf:about="&edxl_cap;webInfo">
        <rdfs:comment xml:lang="en">The identifier of the hyperlink associating additional information with the alert message</rdfs:comment>
        <rdfs:domain rdf:resource="&edxl_cap;Info"/>
        <rdfs:range rdf:resource="&xsd;string"/>
    </owl:DatatypeProperty>
    


    <!-- 
    ///////////////////////////////////////////////////////////////////////////////////////
    //
    // Classes
    //
    ///////////////////////////////////////////////////////////////////////////////////////
     -->

    


    <!-- http://fpc.ufba.br/ontologies/edxl_cap#AckType -->

    <owl:Class rdf:about="&edxl_cap;AckType">
        <rdfs:subClassOf rdf:resource="&edxl_cap;MsgType"/>
        <owl:disjointWith rdf:resource="&edxl_cap;AlertType"/>
        <owl:disjointWith rdf:resource="&edxl_cap;CancelType"/>
        <owl:disjointWith rdf:resource="&edxl_cap;ErrorType"/>
        <owl:disjointWith rdf:resource="&edxl_cap;UpdateType"/>
        <rdfs:comment xml:lang="en">Acknowledges receipt and acceptance of the message(s) identified in &lt;references&gt;.</rdfs:comment>
        <rdfs:comment xml:lang="pt">Reconhece a recepção e aceitação da mensagem identificada previamente.</rdfs:comment>
    </owl:Class>
    


    <!-- http://fpc.ufba.br/ontologies/edxl_cap#Actual -->

    <owl:Class rdf:about="&edxl_cap;Actual">
        <rdfs:subClassOf rdf:resource="&edxl_cap;Status"/>
        <owl:disjointWith rdf:resource="&edxl_cap;Draft"/>
        <owl:disjointWith rdf:resource="&edxl_cap;Exercise"/>
        <owl:disjointWith rdf:resource="&edxl_cap;System"/>
        <owl:disjointWith rdf:resource="&edxl_cap;Test"/>
        <rdfs:comment xml:lang="en">Actionable by all targeted recipients</rdfs:comment>
        <rdfs:comment xml:lang="pt">Acionável por todos os recipientes-alvo.</rdfs:comment>
    </owl:Class>
    


    <!-- http://fpc.ufba.br/ontologies/edxl_cap#AlertMessage -->

    <owl:Class rdf:about="&edxl_cap;AlertMessage">
        <owl:equivalentClass>
            <owl:Class>
                <owl:intersectionOf rdf:parseType="Collection">
                    <owl:Restriction>
                        <owl:onProperty rdf:resource="&edxl_cap;hasIncidentRelated"/>
                        <owl:someValuesFrom rdf:resource="&edxl_cap;Incident"/>
                    </owl:Restriction>
                    <owl:Restriction>
                        <owl:onProperty rdf:resource="&edxl_cap;hasScope"/>
                        <owl:onClass rdf:resource="&edxl_cap;Scope"/>
                        <owl:maxQualifiedCardinality rdf:datatype="&xsd;nonNegativeInteger">1</owl:maxQualifiedCardinality>
                    </owl:Restriction>
                    <owl:Restriction>
                        <owl:onProperty rdf:resource="&edxl_cap;hasStatus"/>
                        <owl:onClass rdf:resource="&edxl_cap;Status"/>
                        <owl:maxQualifiedCardinality rdf:datatype="&xsd;nonNegativeInteger">1</owl:maxQualifiedCardinality>
                    </owl:Restriction>
                </owl:intersectionOf>
            </owl:Class>
        </owl:equivalentClass>
        <rdfs:comment xml:lang="en">Refers to all component parts of the alert message.</rdfs:comment>
        <rdfs:comment xml:lang="pt">Refere-se todos os componentes da uma mensagem de alerta.  </rdfs:comment>
    </owl:Class>
    


    <!-- http://fpc.ufba.br/ontologies/edxl_cap#AlertType -->

    <owl:Class rdf:about="&edxl_cap;AlertType">
        <rdfs:subClassOf rdf:resource="&edxl_cap;MsgType"/>
        <owl:disjointWith rdf:resource="&edxl_cap;CancelType"/>
        <owl:disjointWith rdf:resource="&edxl_cap;ErrorType"/>
        <owl:disjointWith rdf:resource="&edxl_cap;UpdateType"/>
        <rdfs:comment xml:lang="en">Initial information requiring attention by targeted recipients.</rdfs:comment>
        <rdfs:comment xml:lang="pt">Informação inicial requerendo atenção para os recipientes alvo.</rdfs:comment>
    </owl:Class>
    


    <!-- http://fpc.ufba.br/ontologies/edxl_cap#AllClear -->

    <owl:Class rdf:about="&edxl_cap;AllClear">
        <rdfs:subClassOf rdf:resource="&edxl_cap;ResponseType"/>
        <owl:disjointWith rdf:resource="&edxl_cap;Assess"/>
        <owl:disjointWith rdf:resource="&edxl_cap;Avoid"/>
        <owl:disjointWith rdf:resource="&edxl_cap;Evacuate"/>
        <owl:disjointWith rdf:resource="&edxl_cap;Execute"/>
        <owl:disjointWith rdf:resource="&edxl_cap;Monitor"/>
        <owl:disjointWith rdf:resource="&edxl_cap;None"/>
        <owl:disjointWith rdf:resource="&edxl_cap;Prepare"/>
        <owl:disjointWith rdf:resource="&edxl_cap;Shelter"/>
        <rdfs:comment xml:lang="en">The subject event no longer poses a threat or concern and any follow on action is described in &lt;instruction&gt;</rdfs:comment>
        <rdfs:comment xml:lang="pt">O evento não consiste mais em uma ameaça ou preocupação e qualquer ação a se tomar é descrita através de instruções.</rdfs:comment>
    </owl:Class>
    


    <!-- http://fpc.ufba.br/ontologies/edxl_cap#Area -->

    <owl:Class rdf:about="&edxl_cap;Area">
        <rdfs:comment xml:lang="en">Refers to all component parts of the area subelement of the info subelement of the 
alert message.

</rdfs:comment>
        <rdfs:comment xml:lang="pt">Refere-se a todos os componentes de area do sub-elemento Info do elemento Alerta.</rdfs:comment>
    </owl:Class>
    


    <!-- http://fpc.ufba.br/ontologies/edxl_cap#Assess -->

    <owl:Class rdf:about="&edxl_cap;Assess">
        <rdfs:subClassOf rdf:resource="&edxl_cap;ResponseType"/>
        <owl:disjointWith rdf:resource="&edxl_cap;Avoid"/>
        <owl:disjointWith rdf:resource="&edxl_cap;Evacuate"/>
        <owl:disjointWith rdf:resource="&edxl_cap;Execute"/>
        <owl:disjointWith rdf:resource="&edxl_cap;Monitor"/>
        <owl:disjointWith rdf:resource="&edxl_cap;None"/>
        <owl:disjointWith rdf:resource="&edxl_cap;Prepare"/>
        <owl:disjointWith rdf:resource="&edxl_cap;Shelter"/>
        <rdfs:comment xml:lang="en">Evaluate the information in this message</rdfs:comment>
        <rdfs:comment xml:lang="pt">Avaliar a informação na mensagem.


</rdfs:comment>
    </owl:Class>
    


    <!-- http://fpc.ufba.br/ontologies/edxl_cap#Avoid -->

    <owl:Class rdf:about="&edxl_cap;Avoid">
        <rdfs:subClassOf rdf:resource="&edxl_cap;ResponseType"/>
        <owl:disjointWith rdf:resource="&edxl_cap;Evacuate"/>
        <owl:disjointWith rdf:resource="&edxl_cap;Execute"/>
        <owl:disjointWith rdf:resource="&edxl_cap;Monitor"/>
        <owl:disjointWith rdf:resource="&edxl_cap;None"/>
        <owl:disjointWith rdf:resource="&edxl_cap;Prepare"/>
        <owl:disjointWith rdf:resource="&edxl_cap;Shelter"/>
        <rdfs:comment xml:lang="en">Avoid the subject event as per the &lt;instruction&gt;</rdfs:comment>
        <rdfs:comment xml:lang="pt">Evitar o assunto de um evento de acordo a instruções</rdfs:comment>
    </owl:Class>
    


    <!-- http://fpc.ufba.br/ontologies/edxl_cap#CBRNE -->

    <owl:Class rdf:about="&edxl_cap;CBRNE">
        <rdfs:subClassOf rdf:resource="&edxl_cap;Category"/>
        <rdfs:comment xml:lang="en">Chemical, Biological, Radiological, Nuclear or High-Yield Explosive threat or attack</rdfs:comment>
        <rdfs:comment xml:lang="pt">Ataques e ameaças químicas, biologicas, radiológicas, nucleares ou de explosivos.</rdfs:comment>
    </owl:Class>
    


    <!-- http://fpc.ufba.br/ontologies/edxl_cap#CancelType -->

    <owl:Class rdf:about="&edxl_cap;CancelType">
        <rdfs:subClassOf rdf:resource="&edxl_cap;MsgType"/>
        <owl:disjointWith rdf:resource="&edxl_cap;ErrorType"/>
        <owl:disjointWith rdf:resource="&edxl_cap;UpdateType"/>
        <rdfs:comment xml:lang="en">Cancels the earlier message(s) identified in &lt;references&gt;

</rdfs:comment>
        <rdfs:comment xml:lang="pt">Cancela as mensagens anteriores identificadas por uma referência.</rdfs:comment>
    </owl:Class>
    


    <!-- http://fpc.ufba.br/ontologies/edxl_cap#Category -->

    <owl:Class rdf:about="&edxl_cap;Category">
        <rdfs:comment xml:lang="en">Refers to the category of the subject event of the alert message.

</rdfs:comment>
        <rdfs:comment xml:lang="pt">Refere-se a categoria do assunto do evento do alerta de mensagem.</rdfs:comment>
    </owl:Class>
    


    <!-- http://fpc.ufba.br/ontologies/edxl_cap#Certainty -->

    <owl:Class rdf:about="&edxl_cap;Certainty">
        <rdfs:comment xml:lang="en">The certainty of the subject event of the alert message</rdfs:comment>
    </owl:Class>
    


    <!-- http://fpc.ufba.br/ontologies/edxl_cap#CertaintyUnknown -->

    <owl:Class rdf:about="&edxl_cap;CertaintyUnknown">
        <rdfs:subClassOf rdf:resource="&edxl_cap;Certainty"/>
        <rdfs:comment xml:lang="en">Certainty unknown</rdfs:comment>
    </owl:Class>
    


    <!-- http://fpc.ufba.br/ontologies/edxl_cap#Circle -->

    <owl:Class rdf:about="&edxl_cap;Circle">
        <rdfs:subClassOf rdf:resource="&edxl_cap;Area"/>
        <owl:disjointWith rdf:resource="&edxl_cap;Polygon"/>
        <rdfs:comment xml:lang="en">The paired values of a point and radius delineating the affected area of the alert message.</rdfs:comment>
        <rdfs:comment xml:lang="pt">Os valores emparelhados de um ponto e o raio que delineam a área afetada da mensagem de alerta.</rdfs:comment>
    </owl:Class>
    


    <!-- http://fpc.ufba.br/ontologies/edxl_cap#Draft -->

    <owl:Class rdf:about="&edxl_cap;Draft">
        <rdfs:subClassOf rdf:resource="&edxl_cap;Status"/>
        <owl:disjointWith rdf:resource="&edxl_cap;Exercise"/>
        <owl:disjointWith rdf:resource="&edxl_cap;System"/>
        <owl:disjointWith rdf:resource="&edxl_cap;Test"/>
        <rdfs:comment xml:lang="en">A preliminary template or draft, not actionable in its current form.</rdfs:comment>
        <rdfs:comment xml:lang="pt">Um rascunho preliminar, não acionável em sua forma atual.</rdfs:comment>
    </owl:Class>
    


    <!-- http://fpc.ufba.br/ontologies/edxl_cap#Env -->

    <owl:Class rdf:about="&edxl_cap;Env">
        <rdfs:subClassOf rdf:resource="&edxl_cap;Category"/>
        <rdfs:comment xml:lang="en">Pollution and other environmental</rdfs:comment>
        <rdfs:comment xml:lang="pt">Poluição e outros alerta ambientais</rdfs:comment>
    </owl:Class>
    


    <!-- http://fpc.ufba.br/ontologies/edxl_cap#ErrorType -->

    <owl:Class rdf:about="&edxl_cap;ErrorType">
        <rdfs:subClassOf rdf:resource="&edxl_cap;MsgType"/>
        <owl:disjointWith rdf:resource="&edxl_cap;UpdateType"/>
        <rdfs:comment xml:lang="en">Indicates rejection of the message(s) identified in &lt;references&gt;; explanation SHOULD appear in &lt;note&gt;</rdfs:comment>
        <rdfs:comment xml:lang="pt">Indica rejeição a um mensagem identificada por uma referência.</rdfs:comment>
    </owl:Class>
    


    <!-- http://fpc.ufba.br/ontologies/edxl_cap#Evacuate -->

    <owl:Class rdf:about="&edxl_cap;Evacuate">
        <rdfs:subClassOf rdf:resource="&edxl_cap;ResponseType"/>
        <owl:disjointWith rdf:resource="&edxl_cap;Execute"/>
        <owl:disjointWith rdf:resource="&edxl_cap;Monitor"/>
        <owl:disjointWith rdf:resource="&edxl_cap;None"/>
        <owl:disjointWith rdf:resource="&edxl_cap;Prepare"/>
        <owl:disjointWith rdf:resource="&edxl_cap;Shelter"/>
        <rdfs:comment xml:lang="en">Relocate as instructed in the &lt;instruction&gt;</rdfs:comment>
        <rdfs:comment xml:lang="pt">Realocação de acordo a instruções
</rdfs:comment>
    </owl:Class>
    


    <!-- http://fpc.ufba.br/ontologies/edxl_cap#Execute -->

    <owl:Class rdf:about="&edxl_cap;Execute">
        <rdfs:subClassOf rdf:resource="&edxl_cap;ResponseType"/>
        <owl:disjointWith rdf:resource="&edxl_cap;Monitor"/>
        <owl:disjointWith rdf:resource="&edxl_cap;None"/>
        <owl:disjointWith rdf:resource="&edxl_cap;Prepare"/>
        <owl:disjointWith rdf:resource="&edxl_cap;Shelter"/>
        <rdfs:comment xml:lang="en">Execute a pre-planned activity identified in &lt;instruction&gt;</rdfs:comment>
        <rdfs:comment xml:lang="pt">Executar uma atividade pré-planejada identificada em instruções</rdfs:comment>
    </owl:Class>
    


    <!-- http://fpc.ufba.br/ontologies/edxl_cap#Exercise -->

    <owl:Class rdf:about="&edxl_cap;Exercise">
        <rdfs:subClassOf rdf:resource="&edxl_cap;Status"/>
        <owl:disjointWith rdf:resource="&edxl_cap;System"/>
        <owl:disjointWith rdf:resource="&edxl_cap;Test"/>
        <rdfs:comment xml:lang="en">Actionable only by designated exercise participants; exercise identifier SHOULD appear in &lt;note&gt;</rdfs:comment>
        <rdfs:comment xml:lang="pt">Acionável apenas por participantes designados ao exercício. Um identificador do exercício deve ser incluído.</rdfs:comment>
    </owl:Class>
    


    <!-- http://fpc.ufba.br/ontologies/edxl_cap#Expected -->

    <owl:Class rdf:about="&edxl_cap;Expected">
        <rdfs:subClassOf rdf:resource="&edxl_cap;Urgency"/>
        <owl:disjointWith rdf:resource="&edxl_cap;Future"/>
        <owl:disjointWith rdf:resource="&edxl_cap;Immediate"/>
        <owl:disjointWith rdf:resource="&edxl_cap;Past"/>
        <owl:disjointWith rdf:resource="&edxl_cap;UrgencyUnknown"/>
        <rdfs:comment xml:lang="en">Responsive action SHOULD be taken soon (within next hour)</rdfs:comment>
        <rdfs:comment xml:lang="pt">Ações de resposta devem ser realizadas logo (dentro da próxima hora).</rdfs:comment>
    </owl:Class>
    


    <!-- http://fpc.ufba.br/ontologies/edxl_cap#Extreme -->

    <owl:Class rdf:about="&edxl_cap;Extreme">
        <rdfs:subClassOf rdf:resource="&edxl_cap;Severity"/>
        <owl:disjointWith rdf:resource="&edxl_cap;Minor"/>
        <owl:disjointWith rdf:resource="&edxl_cap;Moderate"/>
        <owl:disjointWith rdf:resource="&edxl_cap;Severe"/>
        <owl:disjointWith rdf:resource="&edxl_cap;SeverityUnknown"/>
        <rdfs:comment xml:lang="en">Extraordinary threat to life or property</rdfs:comment>
        <rdfs:comment xml:lang="pt">Extrema ameaça a vida ou propriedade.</rdfs:comment>
    </owl:Class>
    


    <!-- http://fpc.ufba.br/ontologies/edxl_cap#Fire -->

    <owl:Class rdf:about="&edxl_cap;Fire">
        <rdfs:subClassOf rdf:resource="&edxl_cap;Category"/>
        <rdfs:comment xml:lang="en">Fire suppression and rescue</rdfs:comment>
        <rdfs:comment xml:lang="pt">Extinção de incêndio e resgate.</rdfs:comment>
    </owl:Class>
    


    <!-- http://fpc.ufba.br/ontologies/edxl_cap#Future -->

    <owl:Class rdf:about="&edxl_cap;Future">
        <rdfs:subClassOf rdf:resource="&edxl_cap;Urgency"/>
        <owl:disjointWith rdf:resource="&edxl_cap;Immediate"/>
        <owl:disjointWith rdf:resource="&edxl_cap;Past"/>
        <owl:disjointWith rdf:resource="&edxl_cap;UrgencyUnknown"/>
        <rdfs:comment xml:lang="en">Responsive action SHOULD be taken in the near future</rdfs:comment>
        <rdfs:comment xml:lang="pt">Ações de resposta devem ser tomadas em um futuro próximo.</rdfs:comment>
    </owl:Class>
    


    <!-- http://fpc.ufba.br/ontologies/edxl_cap#Geo -->

    <owl:Class rdf:about="&edxl_cap;Geo">
        <rdfs:subClassOf rdf:resource="&edxl_cap;Category"/>
        <rdfs:comment xml:lang="en">Geophysical (inc. landslide)

</rdfs:comment>
        <rdfs:comment xml:lang="pt">Geofísica (ex: deslizamento)</rdfs:comment>
    </owl:Class>
    


    <!-- http://fpc.ufba.br/ontologies/edxl_cap#Health -->

    <owl:Class rdf:about="&edxl_cap;Health">
        <rdfs:subClassOf rdf:resource="&edxl_cap;Category"/>
        <rdfs:comment xml:lang="en">Medical and public health</rdfs:comment>
        <rdfs:comment xml:lang="pt">Saúde pública</rdfs:comment>
    </owl:Class>
    


    <!-- http://fpc.ufba.br/ontologies/edxl_cap#Immediate -->

    <owl:Class rdf:about="&edxl_cap;Immediate">
        <rdfs:subClassOf rdf:resource="&edxl_cap;Urgency"/>
        <owl:disjointWith rdf:resource="&edxl_cap;Past"/>
        <owl:disjointWith rdf:resource="&edxl_cap;UrgencyUnknown"/>
        <rdfs:comment xml:lang="en">Responsive action SHOULD be taken immediately.</rdfs:comment>
        <rdfs:comment xml:lang="pt">Ações de resposta devem ser realizadas imediatamente.</rdfs:comment>
    </owl:Class>
    


    <!-- http://fpc.ufba.br/ontologies/edxl_cap#Incident -->

    <owl:Class rdf:about="&edxl_cap;Incident">
        <rdfs:comment xml:lang="en">Term referring to occurrences of any scale that may require some form of Emergency Response and Management, and that requires tracking and information exchange. 
“Incident” is viewed from the NIMS Emergency Management perspective as a formal or informal declaration of emergency or disaster by an organization at the state, local, federal level or by a jurisdiction.</rdfs:comment>
        <rdfs:comment xml:lang="pt">Termo que se refere a ocorrências de qualquer escala que pode exigir alguma forma de gerenciamento e resposta à emergência, e que requer acompanhamento e troca de informação. No Sistema Nacional de Gerenciamento de Emergência americano (NIMS), &quot;Incidente&quot; é visto como uma declaração formal ou informal de emergência ou desastre por uma organização de nível local, estadual, federal ou por uma jurisdição.</rdfs:comment>
    </owl:Class>
    


    <!-- http://fpc.ufba.br/ontologies/edxl_cap#Info -->

    <owl:Class rdf:about="&edxl_cap;Info">
        <owl:equivalentClass>
            <owl:Class>
                <owl:intersectionOf rdf:parseType="Collection">
                    <owl:Restriction>
                        <owl:onProperty rdf:resource="&edxl_cap;hasArea"/>
                        <owl:someValuesFrom rdf:resource="&edxl_cap;Area"/>
                    </owl:Restriction>
                    <owl:Restriction>
                        <owl:onProperty rdf:resource="&edxl_cap;hasResource"/>
                        <owl:someValuesFrom rdf:resource="&edxl_cap;Resource"/>
                    </owl:Restriction>
                </owl:intersectionOf>
            </owl:Class>
        </owl:equivalentClass>
        <rdfs:comment xml:lang="en">Refers to all component parts of the info sub-element of the alert message.

</rdfs:comment>
        <rdfs:comment xml:lang="pt">Refere-se a todos os componentes de informações sobre a mensagem de alerta.</rdfs:comment>
    </owl:Class>
    


    <!-- http://fpc.ufba.br/ontologies/edxl_cap#Infra -->

    <owl:Class rdf:about="&edxl_cap;Infra">
        <rdfs:subClassOf rdf:resource="&edxl_cap;Category"/>
        <rdfs:comment xml:lang="en">Utility, telecommunication, other non-transport infrastructure</rdfs:comment>
        <rdfs:comment xml:lang="pt">Utilidades, telecomunicações, outras infraestruturadas não transportadas</rdfs:comment>
    </owl:Class>
    


    <!-- http://fpc.ufba.br/ontologies/edxl_cap#Likely -->

    <owl:Class rdf:about="&edxl_cap;Likely">
        <rdfs:subClassOf rdf:resource="&edxl_cap;Certainty"/>
        <rdfs:comment xml:lang="en">Likely (p &gt; ~50%)</rdfs:comment>
    </owl:Class>
    


    <!-- http://fpc.ufba.br/ontologies/edxl_cap#Met -->

    <owl:Class rdf:about="&edxl_cap;Met">
        <rdfs:subClassOf rdf:resource="&edxl_cap;Category"/>
        <rdfs:comment xml:lang="en">Meteorological (inc. flood)</rdfs:comment>
        <rdfs:comment xml:lang="pt">Metereológica (ex:enchente)

</rdfs:comment>
    </owl:Class>
    


    <!-- http://fpc.ufba.br/ontologies/edxl_cap#Minor -->

    <owl:Class rdf:about="&edxl_cap;Minor">
        <rdfs:subClassOf rdf:resource="&edxl_cap;Severity"/>
        <owl:disjointWith rdf:resource="&edxl_cap;Moderate"/>
        <owl:disjointWith rdf:resource="&edxl_cap;Severe"/>
        <owl:disjointWith rdf:resource="&edxl_cap;SeverityUnknown"/>
        <rdfs:comment xml:lang="en">Minimal threat to life or property</rdfs:comment>
        <rdfs:comment xml:lang="pt">Ameaça mínima a vida ou propriedade.</rdfs:comment>
    </owl:Class>
    


    <!-- http://fpc.ufba.br/ontologies/edxl_cap#Moderate -->

    <owl:Class rdf:about="&edxl_cap;Moderate">
        <rdfs:subClassOf rdf:resource="&edxl_cap;Severity"/>
        <owl:disjointWith rdf:resource="&edxl_cap;Severe"/>
        <owl:disjointWith rdf:resource="&edxl_cap;SeverityUnknown"/>
        <rdfs:comment xml:lang="en">Possible threat to life or property</rdfs:comment>
        <rdfs:comment xml:lang="pt">Possível ameaça a vida ou propriedade.</rdfs:comment>
    </owl:Class>
    


    <!-- http://fpc.ufba.br/ontologies/edxl_cap#Monitor -->

    <owl:Class rdf:about="&edxl_cap;Monitor">
        <rdfs:subClassOf rdf:resource="&edxl_cap;ResponseType"/>
        <owl:disjointWith rdf:resource="&edxl_cap;None"/>
        <owl:disjointWith rdf:resource="&edxl_cap;Prepare"/>
        <owl:disjointWith rdf:resource="&edxl_cap;Shelter"/>
        <rdfs:comment xml:lang="en">Attend to information sources as described in &lt;instruction&gt;</rdfs:comment>
        <rdfs:comment xml:lang="pt">Preocupar-se com fontes de informações como descritas em instruções
</rdfs:comment>
    </owl:Class>
    


    <!-- http://fpc.ufba.br/ontologies/edxl_cap#MsgType -->

    <owl:Class rdf:about="&edxl_cap;MsgType">
        <rdfs:comment xml:lang="en">Refers to the nature of the alert message.

</rdfs:comment>
        <rdfs:comment xml:lang="pt">Refere-se a natureza da mensagem de alerta.</rdfs:comment>
    </owl:Class>
    


    <!-- http://fpc.ufba.br/ontologies/edxl_cap#None -->

    <owl:Class rdf:about="&edxl_cap;None">
        <rdfs:subClassOf rdf:resource="&edxl_cap;ResponseType"/>
        <owl:disjointWith rdf:resource="&edxl_cap;Prepare"/>
        <owl:disjointWith rdf:resource="&edxl_cap;Shelter"/>
        <rdfs:comment xml:lang="en">No action recommended</rdfs:comment>
        <rdfs:comment xml:lang="pt">Nenhuma ação recomendada</rdfs:comment>
    </owl:Class>
    


    <!-- http://fpc.ufba.br/ontologies/edxl_cap#Observed -->

    <owl:Class rdf:about="&edxl_cap;Observed">
        <rdfs:subClassOf rdf:resource="&edxl_cap;Certainty"/>
        <rdfs:comment xml:lang="en">Determined to have occurred or to be ongoing</rdfs:comment>
    </owl:Class>
    


    <!-- http://fpc.ufba.br/ontologies/edxl_cap#OtherCategory -->

    <owl:Class rdf:about="&edxl_cap;OtherCategory">
        <rdfs:subClassOf rdf:resource="&edxl_cap;Category"/>
        <rdfs:comment xml:lang="en">Others events</rdfs:comment>
        <rdfs:comment xml:lang="pt">Outros eventos</rdfs:comment>
    </owl:Class>
    


    <!-- http://fpc.ufba.br/ontologies/edxl_cap#Past -->

    <owl:Class rdf:about="&edxl_cap;Past">
        <rdfs:subClassOf rdf:resource="&edxl_cap;Urgency"/>
        <owl:disjointWith rdf:resource="&edxl_cap;UrgencyUnknown"/>
        <rdfs:comment xml:lang="en">Responsive action is no longer required</rdfs:comment>
        <rdfs:comment xml:lang="pt">Ações de resposta não são mais necessárias.</rdfs:comment>
    </owl:Class>
    


    <!-- http://fpc.ufba.br/ontologies/edxl_cap#Polygon -->

    <owl:Class rdf:about="&edxl_cap;Polygon">
        <rdfs:subClassOf rdf:resource="&edxl_cap;Area"/>
        <rdfs:comment xml:lang="en">The paired values of points defining a polygon that delineates the affected area of the alert message</rdfs:comment>
    </owl:Class>
    


    <!-- http://fpc.ufba.br/ontologies/edxl_cap#Possible -->

    <owl:Class rdf:about="&edxl_cap;Possible">
        <rdfs:subClassOf rdf:resource="&edxl_cap;Certainty"/>
        <rdfs:comment xml:lang="en">Possible but not likely (p &lt;= ~50%)</rdfs:comment>
    </owl:Class>
    


    <!-- http://fpc.ufba.br/ontologies/edxl_cap#Prepare -->

    <owl:Class rdf:about="&edxl_cap;Prepare">
        <rdfs:subClassOf rdf:resource="&edxl_cap;ResponseType"/>
        <owl:disjointWith rdf:resource="&edxl_cap;Shelter"/>
        <rdfs:comment xml:lang="en">Make preparations per the &lt;instruction&gt;</rdfs:comment>
        <rdfs:comment xml:lang="pt">Fazer preparações baseadas em instruções</rdfs:comment>
    </owl:Class>
    


    <!-- http://fpc.ufba.br/ontologies/edxl_cap#Private -->

    <owl:Class rdf:about="&edxl_cap;Private">
        <rdfs:subClassOf rdf:resource="&edxl_cap;Scope"/>
        <owl:disjointWith rdf:resource="&edxl_cap;Public"/>
        <owl:disjointWith rdf:resource="&edxl_cap;Restricted"/>
        <rdfs:comment xml:lang="en">For dissemination only to specified addresses.</rdfs:comment>
        <rdfs:comment xml:lang="pt">Para disseminação apenas para endereços especificados.</rdfs:comment>
    </owl:Class>
    


    <!-- http://fpc.ufba.br/ontologies/edxl_cap#Public -->

    <owl:Class rdf:about="&edxl_cap;Public">
        <rdfs:subClassOf rdf:resource="&edxl_cap;Scope"/>
        <owl:disjointWith rdf:resource="&edxl_cap;Restricted"/>
        <rdfs:comment xml:lang="en">For general dissemination to unrestricted audiences.</rdfs:comment>
        <rdfs:comment xml:lang="pt">Para a divulgação para o público em geral sem restrições</rdfs:comment>
    </owl:Class>
    


    <!-- http://fpc.ufba.br/ontologies/edxl_cap#Rescue -->

    <owl:Class rdf:about="&edxl_cap;Rescue">
        <rdfs:subClassOf rdf:resource="&edxl_cap;Category"/>
        <rdfs:comment xml:lang="en">Rescue and recovery</rdfs:comment>
        <rdfs:comment xml:lang="pt">Resgate e recuperação</rdfs:comment>
    </owl:Class>
    


    <!-- http://fpc.ufba.br/ontologies/edxl_cap#Resource -->

    <owl:Class rdf:about="&edxl_cap;Resource">
        <rdfs:comment xml:lang="en">Refers to an additional file with supplemental information related to this &lt;info&gt; element; e.g., an image or audio file</rdfs:comment>
    </owl:Class>
    


    <!-- http://fpc.ufba.br/ontologies/edxl_cap#ResponseType -->

    <owl:Class rdf:about="&edxl_cap;ResponseType">
        <rdfs:comment xml:lang="en">The code denoting the type of action recommended for the target audience</rdfs:comment>
        <rdfs:comment xml:lang="pt">O tipo de ação recomendada para a audiência alvo da mensagem de alerta.</rdfs:comment>
    </owl:Class>
    


    <!-- http://fpc.ufba.br/ontologies/edxl_cap#Restricted -->

    <owl:Class rdf:about="&edxl_cap;Restricted">
        <rdfs:subClassOf rdf:resource="&edxl_cap;Scope"/>
        <rdfs:comment xml:lang="en">For dissemination only to users with a known operational requirement. </rdfs:comment>
        <rdfs:comment xml:lang="pt">Para disseminação somente para usuários com requerimento operacional conhecido.</rdfs:comment>
    </owl:Class>
    


    <!-- http://fpc.ufba.br/ontologies/edxl_cap#Safety -->

    <owl:Class rdf:about="&edxl_cap;Safety">
        <rdfs:subClassOf rdf:resource="&edxl_cap;Category"/>
        <rdfs:comment xml:lang="en">General emergency and public safety</rdfs:comment>
        <rdfs:comment xml:lang="pt">Emergência geral e segurança pública

</rdfs:comment>
    </owl:Class>
    


    <!-- http://fpc.ufba.br/ontologies/edxl_cap#Scope -->

    <owl:Class rdf:about="&edxl_cap;Scope">
        <rdfs:comment xml:lang="en">Refers to the intended distribution of the alert message.

</rdfs:comment>
        <rdfs:comment xml:lang="pt">Refere-se a intenção da distribuição da mensagem de alerta.</rdfs:comment>
    </owl:Class>
    


    <!-- http://fpc.ufba.br/ontologies/edxl_cap#Security -->

    <owl:Class rdf:about="&edxl_cap;Security">
        <rdfs:subClassOf rdf:resource="&edxl_cap;Category"/>
        <rdfs:comment xml:lang="en">Law enforcement, military, homeland and local/private security</rdfs:comment>
        <rdfs:comment xml:lang="pt">Aplicações da lei, militares, segurança nacional e local/privada</rdfs:comment>
    </owl:Class>
    


    <!-- http://fpc.ufba.br/ontologies/edxl_cap#Sender -->

    <owl:Class rdf:about="&edxl_cap;Sender">
        <rdfs:comment xml:lang="en">The originator of an alert. Guaranteed by assigner to be unique globally; e.g., may be based on an Internet domain name.</rdfs:comment>
    </owl:Class>
    


    <!-- http://fpc.ufba.br/ontologies/edxl_cap#Severe -->

    <owl:Class rdf:about="&edxl_cap;Severe">
        <rdfs:subClassOf rdf:resource="&edxl_cap;Severity"/>
        <owl:disjointWith rdf:resource="&edxl_cap;SeverityUnknown"/>
        <rdfs:comment xml:lang="en">Significant threat to life or property</rdfs:comment>
        <rdfs:comment xml:lang="pt">Significante ameaça a vida ou propriedade.</rdfs:comment>
    </owl:Class>
    


    <!-- http://fpc.ufba.br/ontologies/edxl_cap#Severity -->

    <owl:Class rdf:about="&edxl_cap;Severity">
        <rdfs:comment xml:lang="en">The severity of the subject incident or event.
</rdfs:comment>
    </owl:Class>
    


    <!-- http://fpc.ufba.br/ontologies/edxl_cap#SeverityUnknown -->

    <owl:Class rdf:about="&edxl_cap;SeverityUnknown">
        <rdfs:subClassOf rdf:resource="&edxl_cap;Severity"/>
        <rdfs:comment xml:lang="en">Severity unknown</rdfs:comment>
    </owl:Class>
    


    <!-- http://fpc.ufba.br/ontologies/edxl_cap#Shelter -->

    <owl:Class rdf:about="&edxl_cap;Shelter">
        <rdfs:subClassOf rdf:resource="&edxl_cap;ResponseType"/>
        <rdfs:comment xml:lang="en">Take shelter in place or per &lt;instruction&gt;
</rdfs:comment>
        <rdfs:comment xml:lang="pt">Se abrigar num local ou por instrução
</rdfs:comment>
    </owl:Class>
    


    <!-- http://fpc.ufba.br/ontologies/edxl_cap#Status -->

    <owl:Class rdf:about="&edxl_cap;Status">
        <rdfs:comment xml:lang="en">Refers to the appropriate handling of the alert message. </rdfs:comment>
        <rdfs:comment xml:lang="pt">Refere-se ao modo apropriado para lidar com o tipo de mensagem de alerta.</rdfs:comment>
    </owl:Class>
    


    <!-- http://fpc.ufba.br/ontologies/edxl_cap#System -->

    <owl:Class rdf:about="&edxl_cap;System">
        <rdfs:subClassOf rdf:resource="&edxl_cap;Status"/>
        <owl:disjointWith rdf:resource="&edxl_cap;Test"/>
        <rdfs:comment xml:lang="en">For messages that support alert network internal functions.</rdfs:comment>
        <rdfs:comment xml:lang="pt">Para mensagens que apoiam funções internas da rede de alerta.</rdfs:comment>
    </owl:Class>
    


    <!-- http://fpc.ufba.br/ontologies/edxl_cap#Test -->

    <owl:Class rdf:about="&edxl_cap;Test">
        <rdfs:subClassOf rdf:resource="&edxl_cap;Status"/>
        <rdfs:comment xml:lang="en">Technical testing only, all recipients disregard.</rdfs:comment>
        <rdfs:comment xml:lang="pt">Testes técnicos, todos os recipientes não são levados em consideração.</rdfs:comment>
    </owl:Class>
    


    <!-- http://fpc.ufba.br/ontologies/edxl_cap#Transport -->

    <owl:Class rdf:about="&edxl_cap;Transport">
        <rdfs:subClassOf rdf:resource="&edxl_cap;Category"/>
        <rdfs:comment xml:lang="en">Public and private transportation</rdfs:comment>
        <rdfs:comment xml:lang="pt">Transporte público e privado.</rdfs:comment>
    </owl:Class>
    


    <!-- http://fpc.ufba.br/ontologies/edxl_cap#Unlikely -->

    <owl:Class rdf:about="&edxl_cap;Unlikely">
        <rdfs:subClassOf rdf:resource="&edxl_cap;Certainty"/>
        <rdfs:comment xml:lang="en">Not expected to occur (p ~ 0)</rdfs:comment>
    </owl:Class>
    


    <!-- http://fpc.ufba.br/ontologies/edxl_cap#UpdateType -->

    <owl:Class rdf:about="&edxl_cap;UpdateType">
        <rdfs:subClassOf rdf:resource="&edxl_cap;MsgType"/>
        <rdfs:comment xml:lang="en">Updates and supercedes the earlier message(s) identified in &lt;references&gt;</rdfs:comment>
        <rdfs:comment xml:lang="pt">Atualiza ou sobrepõe mensagens anteriores identificadas por uma referência.</rdfs:comment>
    </owl:Class>
    


    <!-- http://fpc.ufba.br/ontologies/edxl_cap#Urgency -->

    <owl:Class rdf:about="&edxl_cap;Urgency">
        <rdfs:comment xml:lang="en">The urgency of the subject event of the alert message</rdfs:comment>
    </owl:Class>
    


    <!-- http://fpc.ufba.br/ontologies/edxl_cap#UrgencyUnknown -->

    <owl:Class rdf:about="&edxl_cap;UrgencyUnknown">
        <rdfs:subClassOf rdf:resource="&edxl_cap;Urgency"/>
        <rdfs:comment xml:lang="en">Urgency not known</rdfs:comment>
        <rdfs:comment xml:lang="pt">Urgência desconhecida</rdfs:comment>
    </owl:Class>
</rdf:RDF>



<!-- Generated by the OWL API (version 3.4.2) http://owlapi.sourceforge.net -->

