
@prefix owl: <http://www.w3.org/2002/07/owl#> .
@prefix xsd: <http://www.w3.org/2001/XMLSchema#> .
@prefix rdfs: <http://www.w3.org/2000/01/rdf-schema#> .
@prefix : <http://ontology.universAAL.org/uAAL.owl#> .
<http://ontology.universAAL.org/DataRepresentation.owl> rdfs:comment "Ontology of the universAAL Basic Data Representation Model"^^xsd:string ;
  a owl:Ontology ;
  rdfs:label "Basic Data Representation Model"^^xsd:string .
:ManagedIndividual rdfs:comment "The root of the whole class hierarchy in the uAAL ontology."^^xsd:string ;
  a owl:Class ;
  rdfs:label "uAAL Ontology Root Class"^^xsd:string .
:ComparableIndividual rdfs:comment "The root class for all comparable individuals in the uAAL ontology."^^xsd:string ;
  a owl:Class ;
  rdfs:label "Comparable Individual"^^xsd:string ;
  rdfs:subClassOf :ManagedIndividual .
:LevelRating rdfs:comment "An enumeration for specifying the level of appearance / availability of a phenomen."^^xsd:string ;
  a owl:Class ;
  rdfs:label "Level Rating"^^xsd:string ;
  rdfs:subClassOf :ComparableIndividual ;
  owl:oneOf (
    :none
    :low
    :middle
    :high
    :full
  ) .
:full a :LevelRating .
:middle a :LevelRating .
:high a :LevelRating .
:low a :LevelRating .
:none a :LevelRating .
:AbsLocation rdfs:comment "The root class for all locations."^^xsd:string ;
  a owl:Class ;
  rdfs:label "Abstract Location"^^xsd:string ;
  rdfs:subClassOf :ComparableIndividual .
:PrivateResource rdfs:comment "An abstract superclass that ManagedIndividuals can subclass to indicate they represent private data"^^xsd:string ;
  a owl:Class ;
  rdfs:label "Private Resource"^^xsd:string ;
  rdfs:subClassOf :ManagedIndividual .
:Rating rdfs:comment "An enumeration for rating the perceived quality of a service similar to the german marks system for students' work."^^xsd:string ;
  a owl:Class ;
  rdfs:label "QoS Rating"^^xsd:string ;
  rdfs:subClassOf :ComparableIndividual ;
  owl:oneOf (
    :poor
    :almost_poor
    :almost_sufficient
    :sufficient
    :rich_sufficient
    :almost_satisfying
    :satisfying
    :rich_satisfying
    :almost_good
    :good
    :rich_good
    :almost_excellent
    :excellent
  ) .
:poor a :Rating .
:rich_sufficient a :Rating .
:rich_satisfying a :Rating .
:almost_satisfying a :Rating .
:sufficient a :Rating .
:excellent a :Rating .
:almost_excellent a :Rating .
:satisfying a :Rating .
:almost_poor a :Rating .
:rich_good a :Rating .
:almost_good a :Rating .
:good a :Rating .
:almost_sufficient a :Rating .
<http://ontology.universAAL.org/Service.owl#PropertyPath> a rdfs:class .
